updated the world changes lemmas to now also revoke Monotemporary, proved lemmas about batch uninitializing all addresses above a certain address

theories/examples/contiguous.v
@@ -498,6 +498,14 @@ Section Contiguous.
       eapply contiguous_between_cons; eauto. }
   Qed.
 
+  Lemma contiguous_between_weak a a1 b e l:
+    contiguous_between (a :: a1 :: l) b e →
+    contiguous_between (a1 :: l) a1 e.
+  Proof.
+    intros. edestruct contiguous_between_cons_inv as [_ [a' [_ Hcontn] ] ].
+    apply H. by destruct (contiguous_between_cons_inv_first _ _ _ _ Hcontn).
+  Qed.
+
 
   Context {Σ:gFunctors} {memg:memG Σ} {regg:regG Σ}
           {stsg : STSG Addr region_type Σ} {heapg : heapG Σ}
@@ -574,52 +582,3 @@ Section Contiguous.
 End Contiguous.
 
 Opaque contiguous.
-
-Definition isCorrectPC_range p g b e a0 an :=
-  ∀ ai, (a0 <= ai)%a ∧ (ai < an)%a → isCorrectPC (inr (p, g, b, e, ai)).
-
-Lemma isCorrectPC_inrange p g b (e a0 an a: Addr) :
-  isCorrectPC_range p g b e a0 an →
-  (a0 <= a < an)%Z →
-  isCorrectPC (inr (p, g, b, e, a)).
-Proof.
-  unfold isCorrectPC_range. move=> /(_ a) HH ?. apply HH. eauto.
-Qed.
-
-Lemma isCorrectPC_contiguous_range p g b e a0 an a l :
-  isCorrectPC_range p g b e a0 an →
-  contiguous_between l a0 an →
-  a ∈ l →
-  isCorrectPC (inr (p, g, b, e, a)).
-Proof.
-  intros Hr Hc Hin.
-  eapply isCorrectPC_inrange; eauto.
-  eapply contiguous_between_middle_bounds'; eauto.
-Qed.
-
-Lemma isCorrectPC_range_perm p g b e a0 an :
-  isCorrectPC_range p g b e a0 an →
-  (a0 < an)%a →
-  p = RX ∨ p = RWX ∨ p = RWLX.
-Proof.
-  intros Hr H0n.
-  assert (isCorrectPC (inr (p, g, b, e, a0))) as HH by (apply Hr; solve_addr).
-  inversion HH; auto.
-Qed.
-
-Lemma isCorrectPC_range_perm_non_E p g b e a0 an :
-  isCorrectPC_range p g b e a0 an →
-  (a0 < an)%a →
-  p ≠ E.
-Proof.
-  intros HH1 HH2. pose proof (isCorrectPC_range_perm _ _ _ _ _ _ HH1 HH2).
-  naive_solver.
-Qed.
-
-Lemma isCorrectPC_range_restrict p g b e a0 an a0' an' :
-  isCorrectPC_range p g b e a0 an →
-  (a0 <= a0')%a ∧ (an' <= an)%a →
-  isCorrectPC_range p g b e a0' an'.
-Proof.
-  intros HR [? ?] a' [? ?]. apply HR. solve_addr.
-Qed.
