theories/examples/macros/checkbelow.v
@@ -1,0 +1,660 @@
+From iris.algebra Require Import frac.
+From iris.proofmode Require Import tactics.
+Require Import Eqdep_dec List.
+From cap_machine Require Import rules.
+From cap_machine Require Export iris_extra addr_reg_sample region_macros contiguous stack_macros_helpers req.
+
+Section stack_macros.
+  Context {Σ:gFunctors} {memg:memG Σ} {regg:regG Σ}
+          `{MonRef: MonRefG (leibnizO _) CapR_rtc Σ}
+          `{MP: MachineParameters}.
+
+
+  (* -------------------------------------- CHECKBELOW ------------------------------------ *)
+  (* the following macro checks that the upper read bound of one capability is below the lower
+     bound of another capability *)
+  (* the macro branches based on the U of the capability *)
+
+  Definition branchperm_instrs_pre r off_to_blockU off_to_skip_blockU :=
+    [move_r r_t3 PC;
+    lea_z r_t3 (off_to_blockU + off_to_skip_blockU);
+    getp r_t1 r;
+    sub_r_z r_t2 r_t1 (encodePerm URW);
+    move_r r_t4 PC;
+    lea_z r_t4 4;
+    jnz r_t4 r_t2; (* if the permission is not URW, we must continue and skip the following jmp *)
+    jmp r_t3;
+    sub_r_z r_t2 r_t1 (encodePerm URWL);
+    lea_z r_t4 4;
+    jnz r_t4 r_t2; (* if the permission is not URWL, we must continue and skip the following jmp *)
+    jmp r_t3;
+    sub_r_z r_t2 r_t1 (encodePerm URWX);
+    lea_z r_t4 4;
+    jnz r_t4 r_t2; (* if the permission is not URWX, we must continue and skip the following jmp *)
+    jmp r_t3;
+    sub_r_z r_t2 r_t1 (encodePerm URWLX);
+    lea_z r_t4 4;
+    jnz r_t4 r_t2; (* if the permission is not URWLX, we must continue and skip the following jmp *)
+    jmp r_t3].
+
+  (* after the above macro, the PC will either point to the instruction right after, or the instruction
+     skipping an offset *)
+
+  Local Definition off_to_blockU := length (branchperm_instrs_pre r_t0 0 0).
+
+  Definition branchperm_instrs r off_to_skip_blockU := branchperm_instrs_pre r off_to_blockU off_to_skip_blockU.
+
+  Definition branchperm r off_to_skip_blockU a p : iProp Σ :=
+    ([∗ list] a_i;w_i ∈ a;(branchperm_instrs r off_to_skip_blockU), a_i ↦ₐ[p] w_i)%I.
+
+  Definition isU_word (w : Word) :=
+    match w with
+    | inl _ => false
+    | inr (p,_,_,_,_) => isU p
+    end.
+
+  Lemma branchperm_spec r a w pc_p pc_p' pc_g pc_b pc_e a_first a_last a_blockU off_to_skip_blockU φ :
+    isCorrectPC_range pc_p pc_g pc_b pc_e a_first a_last ->
+    PermFlows pc_p pc_p' ->
+    contiguous_between a a_first a_last ->
+    (a_first + (off_to_blockU + off_to_skip_blockU))%a = Some a_blockU →
+
+      ▷ branchperm r off_to_skip_blockU a pc_p'
+    ∗ ▷ PC ↦ᵣ inr (pc_p,pc_g,pc_b,pc_e,a_first)
+    ∗ ▷ r ↦ᵣ w
+    ∗ ▷ (∃ w, r_t1 ↦ᵣ w)
+    ∗ ▷ (∃ w, r_t2 ↦ᵣ w)
+    ∗ ▷ (∃ w, r_t3 ↦ᵣ w)
+    ∗ ▷ (∃ w, r_t4 ↦ᵣ w)
+    ∗ ▷ (if is_cap w then
+           ∃ l p b e a', ⌜w = inr (p,l,b,e,a')⌝ ∧
+           if isU p then
+             (PC ↦ᵣ inr (pc_p,pc_g,pc_b,pc_e,a_blockU) ∗ branchperm r off_to_skip_blockU a pc_p' ∗
+                 r ↦ᵣ inr (p,l,b,e,a') ∗ (∃ w, r_t1 ↦ᵣ w) ∗ (∃ w, r_t2 ↦ᵣ w) ∗ (∃ w, r_t3 ↦ᵣ w) ∗ (∃ w, r_t4 ↦ᵣ w)
+                 -∗ WP Seq (Instr Executable) {{ φ }})
+           else
+             (PC ↦ᵣ inr (pc_p,pc_g,pc_b,pc_e,a_last) ∗ branchperm r off_to_skip_blockU a pc_p' ∗
+                 r ↦ᵣ inr (p,l,b,e,a') ∗ (∃ w, r_t1 ↦ᵣ w) ∗ (∃ w, r_t2 ↦ᵣ w) ∗ (∃ w, r_t3 ↦ᵣ w) ∗ (∃ w, r_t4 ↦ᵣ w)
+                 -∗ WP Seq (Instr Executable) {{ φ }})
+        else φ FailedV)
+    ⊢
+      WP Seq (Instr Executable) {{ φ }}.
+  Proof.
+    iIntros (Hvpc Hfl Hcont Hoff) "(>Hprog & >HPC & >Hr & >Hr_t1 & >Hr_t2 & Hr_t3 & Hr_t4 & Hcont)".
+    iDestruct (big_sepL2_length with "Hprog") as %Hlength. simpl in *.
+    iDestruct ("Hr_t1") as (w1) "Hr_t1".
+    iDestruct ("Hr_t2") as (w2) "Hr_t2".
+    iDestruct ("Hr_t3") as (w3) "Hr_t3".
+    iDestruct ("Hr_t4") as (w4) "Hr_t4".
+    prep_addr_list_full a Hcont.
+    assert (pc_p ≠ E) as Hnp.
+    { eapply pc_range_not_E;eauto. }
+    pose proof (pc_range_perm _ _ _ _ _ _ _ Hvpc Hcont) as Hperms.
+    iAssert (⌜r ≠ PC⌝)%I as %Hne.
+    { destruct (decide (r = PC)); auto; subst. iDestruct (regname_dupl_false with "HPC Hr") as %Hcontr. done. }
+    (* move_r r_t3 PC *)
+    iPrologue "Hprog".
+    iApply (wp_move_success_reg_fromPC with "[$Hi $HPC $Hr_t3]");
+      [apply decode_encode_instrW_inv|auto|iCorrectPC a_first a_last|iContiguous_next_a Hcont|..].
+    iEpilogue "(HPC & Hprog_done & Hr_t3)".
+    (* lea r_t3 (off1 + off2) *)
+    iPrologue "Hprog".
+    iApply (wp_lea_success_z with "[$Hi $HPC $Hr_t3]");
+      [apply decode_encode_instrW_inv|auto|iCorrectPC a_first a_last|iContiguous_next_a Hcont|apply Hoff|auto..].
+    { destruct Hperms as [-> | [-> | ->] ]; auto. }
+    iEpilogue "(HPC & Hi & Hr_t3)";iCombine "Hi" "Hprog_done" as "Hprog_done".
+    (* getp r_t1 r *)
+    iPrologue "Hprog".
+    destruct w.
+    { (* if w is an integer, the getL will fail *)
+      iApply (wp_Get_fail with "[$HPC $Hi $Hr_t1 $Hr]");
+        [apply decode_encode_instrW_inv|auto|apply Hfl|iCorrectPC a_first a_last|..].
+      iEpilogue "_ /=".
+      iApply wp_value. done. }
+    destruct c,p,p,p.
+    iApply (wp_Get_success with "[$HPC $Hi $Hr $Hr_t1]");
+      [apply decode_encode_instrW_inv|auto|auto|iCorrectPC a_first a_last|iContiguous_next_a Hcont|auto..].
+    iEpilogue "(HPC & Hi & Hr & Hr_t1)";iCombine "Hi" "Hprog_done" as "Hprog_done".
+    iSimpl in "Hr_t1".
+    (* sub r_t2 r_t1 URW *)
+    iPrologue "Hprog".
+    iApply (wp_add_sub_lt_success_r_z with "[$HPC $Hi $Hr_t2 $Hr_t1]");
+      [apply decode_encode_instrW_inv|eauto|iContiguous_next_a Hcont|auto|iCorrectPC a_first a_last|..].
+    iEpilogue "(HPC & Hi & Hr_t1 & Hr_t2)";iCombine "Hi" "Hprog_done" as "Hprog_done".
+    (* move r_t4 PC *)
+    iPrologue "Hprog".
+    iApply (wp_move_success_reg_fromPC with "[$Hi $HPC $Hr_t4]");
+      [apply decode_encode_instrW_inv|auto|iCorrectPC a_first a_last|iContiguous_next_a Hcont|..].
+    iEpilogue "(HPC & Hi & Hr_t4)";iCombine "Hi" "Hprog_done" as "Hprog_done".
+    (* lea r_t4 4 *)
+    assert (a3 + 4 = Some a7)%a as Hlea.
+    { apply contiguous_between_incr_addr_middle with (i:=4) (j:=4) (ai:=a3) (aj:=a7) in Hcont;auto. }
+    iPrologue "Hprog".
+    iApply (wp_lea_success_z with "[$Hi $HPC $Hr_t4]");
+      [apply decode_encode_instrW_inv|auto|iCorrectPC a_first a_last|iContiguous_next_a Hcont|apply Hlea|auto..].
+    { destruct Hperms as [-> | [-> | ->] ]; auto. }
+    iEpilogue "(HPC & Hi & Hr_t4)";iCombine "Hi" "Hprog_done" as "Hprog_done".
+    (* jnz r_t4 r_t2 *)
+    iPrologue "Hprog". iSimpl in "Hr_t2".
+    destruct (decide (encodePerm p - encodePerm URW = 0)%Z).
+    { (* if the permission is URW we are done and will jump to the last block *)
+      rewrite e.
+      iApply (wp_jnz_success_next with "[$Hi $HPC $Hr_t4 $Hr_t2]");
+        [apply decode_encode_instrW_inv|auto|iCorrectPC a_first a_last|iContiguous_next_a Hcont|..].
+      iEpilogue "(HPC & Hi & Hr_t4 & Hr_t2)";iCombine "Hi" "Hprog_done" as "Hprog_done".
+      (* jmp r_t3 *)
+      iPrologue "Hprog".
+      iApply (wp_jmp_success with "[$Hi $Hr_t3 $HPC]");
+        [apply decode_encode_instrW_inv|auto|iCorrectPC a_first a_last|auto|..].
+      iEpilogue "(HPC & Hi & Hr_t3)";iCombine "Hi" "Hprog_done" as "Hprog_done".
+      (* Hφ *)
+      assert (p = URW);[apply encodePerm_inj;lia|subst p]. iSimpl in "Hcont".
+      iDestruct "Hcont" as (l0 p b e0 a' Heq) "Hφ". simplify_eq. iSimpl in "Hφ".
+      iApply "Hφ". rewrite updatePcPerm_cap_non_E//. iFrame "HPC Hr".
+      iSplitL "Hprog Hprog_done".
+      { iFrame. iDestruct "Hprog_done" as "($&$&$&$&$&$&$&$)". }
+      iSplitL "Hr_t1";[eauto|]. iSplitL "Hr_t2";[eauto|]. iSplitL "Hr_t3";eauto. 
+    }
+    (* otherwise we keep checking *)
+    iApply (wp_jnz_success_jmp with "[$Hi $HPC $Hr_t4 $Hr_t2]");
+      [apply decode_encode_instrW_inv|auto|iCorrectPC a_first a_last|intros;congruence|..].
+    iEpilogue "(HPC & Hi & Hr_t4 & Hr_t2)";iCombine "Hi" "Hprog_done" as "Hprog_done".
+    iDestruct "Hprog" as "[Hi Hprog]";iCombine "Hi" "Hprog_done" as "Hprog_done".
+    (* sub r_t2 r_t1 URWL *)
+    rewrite updatePcPerm_cap_non_E//.
+    iPrologue "Hprog".
+    iApply (wp_add_sub_lt_success_r_z with "[$HPC $Hi $Hr_t1 $Hr_t2]");
+      [apply decode_encode_instrW_inv|eauto|iContiguous_next_a Hcont|auto|iCorrectPC a_first a_last|..].
+    iEpilogue "(HPC & Hi & Hr_t1 & Hr_t2)";iCombine "Hi" "Hprog_done" as "Hprog_done".
+    (* lea r_t4 4 *)
+    assert (a7 + 4 = Some a11)%a as Hlea'.
+    { apply contiguous_between_incr_addr_middle with (i:=8) (j:=4) (ai:=a7) (aj:=a11) in Hcont;auto. }
+    iPrologue "Hprog".
+    iApply (wp_lea_success_z with "[$Hi $HPC $Hr_t4]");
+      [apply decode_encode_instrW_inv|auto|iCorrectPC a_first a_last|iContiguous_next_a Hcont|apply Hlea'|auto..].
+    { destruct Hperms as [-> | [-> | ->] ]; auto. }
+    iEpilogue "(HPC & Hi & Hr_t4)";iCombine "Hi" "Hprog_done" as "Hprog_done".
+    (* jnz r_t4 r_t2 *)
+    iPrologue "Hprog". iSimpl in "Hr_t2".
+    destruct (decide (encodePerm p - encodePerm URWL = 0)%Z).
+    { (* if the permission is URW we are done and will jump to the last block *)
+      rewrite e.
+      iApply (wp_jnz_success_next with "[$Hi $HPC $Hr_t4 $Hr_t2]");
+        [apply decode_encode_instrW_inv|auto|iCorrectPC a_first a_last|iContiguous_next_a Hcont|..].
+      iEpilogue "(HPC & Hi & Hr_t4 & Hr_t2)";iCombine "Hi" "Hprog_done" as "Hprog_done".
+      (* jmp r_t3 *)
+      iPrologue "Hprog".
+      iApply (wp_jmp_success with "[$Hi $Hr_t3 $HPC]");
+        [apply decode_encode_instrW_inv|auto|iCorrectPC a_first a_last|auto|..].
+      iEpilogue "(HPC & Hi & Hr_t3)";iCombine "Hi" "Hprog_done" as "Hprog_done".
+      (* Hφ *)
+      assert (p = URWL);[apply encodePerm_inj;lia|subst p]. iSimpl in "Hcont".
+      iDestruct "Hcont" as (l0 p b e0 a' Heq) "Hφ". simplify_eq. iSimpl in "Hφ".
+      iApply "Hφ". rewrite updatePcPerm_cap_non_E//. iFrame "HPC Hr".
+      iSplitL "Hprog Hprog_done".
+      { iFrame. iDestruct "Hprog_done" as "($&$&$&$&$&$&$&$&$&$&$&$)". }
+      iSplitL "Hr_t1";[eauto|]. iSplitL "Hr_t2";[eauto|]. iSplitL "Hr_t3";eauto. 
+    }
+    (* otherwise we keep checking *)
+    iApply (wp_jnz_success_jmp with "[$Hi $HPC $Hr_t4 $Hr_t2]");
+      [apply decode_encode_instrW_inv|auto|iCorrectPC a_first a_last|intros;congruence|..].
+    iEpilogue "(HPC & Hi & Hr_t4 & Hr_t2)";iCombine "Hi" "Hprog_done" as "Hprog_done".
+    iDestruct "Hprog" as "[Hi Hprog]";iCombine "Hi" "Hprog_done" as "Hprog_done".
+    rewrite updatePcPerm_cap_non_E//.
+    (* sub r_t2 r_t1 URWL *)
+    iPrologue "Hprog".
+    iApply (wp_add_sub_lt_success_r_z with "[$HPC $Hi $Hr_t1 $Hr_t2]");
+      [apply decode_encode_instrW_inv|eauto|iContiguous_next_a Hcont|auto|iCorrectPC a_first a_last|..].
+    iEpilogue "(HPC & Hi & Hr_t1 & Hr_t2)";iCombine "Hi" "Hprog_done" as "Hprog_done".
+    (* lea r_t4 4 *)
+    assert (a11 + 4 = Some a15)%a as Hlea''.
+    { apply contiguous_between_incr_addr_middle with (i:=12) (j:=4) (ai:=a11) (aj:=a15) in Hcont;auto. }
+    iPrologue "Hprog".
+    iApply (wp_lea_success_z with "[$Hi $HPC $Hr_t4]");
+      [apply decode_encode_instrW_inv|auto|iCorrectPC a_first a_last|iContiguous_next_a Hcont|apply Hlea''|auto..].
+    { destruct Hperms as [-> | [-> | ->] ]; auto. }
+    iEpilogue "(HPC & Hi & Hr_t4)";iCombine "Hi" "Hprog_done" as "Hprog_done".
+    (* jnz r_t4 r_t2 *)
+    iPrologue "Hprog". iSimpl in "Hr_t2".
+    destruct (decide (encodePerm p - encodePerm URWX = 0)%Z).
+    { (* if the permission is URW we are done and will jump to the last block *)
+      rewrite e.
+      iApply (wp_jnz_success_next with "[$Hi $HPC $Hr_t4 $Hr_t2]");
+        [apply decode_encode_instrW_inv|auto|iCorrectPC a_first a_last|iContiguous_next_a Hcont|..].
+      iEpilogue "(HPC & Hi & Hr_t4 & Hr_t2)";iCombine "Hi" "Hprog_done" as "Hprog_done".
+      (* jmp r_t3 *)
+      iPrologue "Hprog".
+      iApply (wp_jmp_success with "[$Hi $Hr_t3 $HPC]");
+        [apply decode_encode_instrW_inv|auto|iCorrectPC a_first a_last|auto|..].
+      iEpilogue "(HPC & Hi & Hr_t3)";iCombine "Hi" "Hprog_done" as "Hprog_done".
+      (* Hφ *)
+      assert (p = URWX);[apply encodePerm_inj;lia|subst p]. iSimpl in "Hcont".
+      iDestruct "Hcont" as (l0 p b e0 a' Heq) "Hφ". simplify_eq. iSimpl in "Hφ".
+      iApply "Hφ". rewrite updatePcPerm_cap_non_E//. iFrame "HPC Hr".
+      iSplitL "Hprog Hprog_done".
+      { iFrame. iDestruct "Hprog_done" as "($&$&$&$&$&$&$&$&$&$&$&$&$&$&$&$)". }
+      iSplitL "Hr_t1";[eauto|]. iSplitL "Hr_t2";[eauto|]. iSplitL "Hr_t3";eauto. 
+    }
+    (* otherwise we keep checking *)
+    iApply (wp_jnz_success_jmp with "[$Hi $HPC $Hr_t4 $Hr_t2]");
+      [apply decode_encode_instrW_inv|auto|iCorrectPC a_first a_last|intros;congruence|..].
+    iEpilogue "(HPC & Hi & Hr_t4 & Hr_t2)";iCombine "Hi" "Hprog_done" as "Hprog_done".
+    iDestruct "Hprog" as "[Hi Hprog]";iCombine "Hi" "Hprog_done" as "Hprog_done".
+    rewrite updatePcPerm_cap_non_E//.
+    (* sub r_t2 r_t1 URWL *)
+    iPrologue "Hprog".
+    iApply (wp_add_sub_lt_success_r_z with "[$HPC $Hi $Hr_t1 $Hr_t2]");
+      [apply decode_encode_instrW_inv|eauto|iContiguous_next_a Hcont|auto|iCorrectPC a_first a_last|..].
+    iEpilogue "(HPC & Hi & Hr_t1 & Hr_t2)";iCombine "Hi" "Hprog_done" as "Hprog_done".
+    (* lea r_t4 4 *)
+    assert (a15 + 4 = Some a_last)%a as Hlea'''.
+    { apply contiguous_between_middle_to_end with (i:=16) (k:=4) (ai:=a15) in Hcont;auto. }
+    iPrologue "Hprog".
+    iApply (wp_lea_success_z with "[$Hi $HPC $Hr_t4]");
+      [apply decode_encode_instrW_inv|auto|iCorrectPC a_first a_last|iContiguous_next_a Hcont|apply Hlea'''|auto..].
+    { destruct Hperms as [-> | [-> | ->] ]; auto. }
+    iEpilogue "(HPC & Hi & Hr_t4)";iCombine "Hi" "Hprog_done" as "Hprog_done".
+    (* jnz r_t4 r_t2 *)
+    iPrologue "Hprog". iSimpl in "Hr_t2".
+    destruct (decide (encodePerm p - encodePerm URWLX = 0)%Z).
+    { (* if the permission is URW we are done and will jump to the last block *)
+      rewrite e.
+      iApply (wp_jnz_success_next with "[$Hi $HPC $Hr_t4 $Hr_t2]");
+        [apply decode_encode_instrW_inv|auto|iCorrectPC a_first a_last|iContiguous_next_a Hcont|..].
+      iEpilogue "(HPC & Hi & Hr_t4 & Hr_t2)";iCombine "Hi" "Hprog_done" as "Hprog_done".
+      (* jmp r_t3 *)
+      iPrologue "Hprog".
+      iApply (wp_jmp_success with "[$Hi $Hr_t3 $HPC]");
+        [apply decode_encode_instrW_inv|auto|iCorrectPC a_first a_last|auto|..].
+      iEpilogue "(HPC & Hi & Hr_t3)";iCombine "Hi" "Hprog_done" as "Hprog_done".
+      (* Hφ *)
+      assert (p = URWLX);[apply encodePerm_inj;lia|subst p]. iSimpl in "Hcont".
+      iDestruct "Hcont" as (l0 p b e0 a' Heq) "Hφ". simplify_eq. iSimpl in "Hφ".
+      iApply "Hφ". rewrite updatePcPerm_cap_non_E//. iFrame "HPC Hr".
+      iSplitL "Hprog Hprog_done".
+      { iFrame. iDestruct "Hprog_done" as "($&$&$&$&$&$&$&$&$&$&$&$&$&$&$&$&$&$&$&$)". }
+      iSplitL "Hr_t1";[eauto|]. iSplitL "Hr_t2";[eauto|]. iSplitL "Hr_t3";eauto.
+    }
+    (* otherwise we go to the first block *)
+    iApply (wp_jnz_success_jmp with "[$Hi $HPC $Hr_t4 $Hr_t2]");
+      [apply decode_encode_instrW_inv|auto|iCorrectPC a_first a_last|intros;congruence|..].
+    iEpilogue "(HPC & Hi & Hr_t4 & Hr_t2)";iCombine "Hi" "Hprog_done" as "Hprog_done".
+    iDestruct "Hprog" as "[Hi Hprog]";iCombine "Hi" "Hprog_done" as "Hprog_done".
+    rewrite updatePcPerm_cap_non_E//.
+    (* Hφ *)
+    iSimpl in "Hcont".
+    iDestruct "Hcont" as (l0 p0 b e a' Heq) "Hcont".
+    simplify_eq.
+    assert (isU p0 = false) as ->.
+    { destruct p0;auto;exfalso;[apply n|apply n0|apply n1|apply n2];clear;lia. }
+    iApply "Hcont".
+    iFrame "Hr HPC".
+    iDestruct "Hprog_done" as "($&$&$&$&$&$&$&$&$&$&$&$&$&$&$&$&$&$&$&$)".
+    iSplit;auto. iSplitL "Hr_t1";[eauto|]. iSplitL "Hr_t2";[eauto|]. iSplitL "Hr_t3";eauto.
+  Qed.
+
+
+  Definition checkbelow_notU_block_instrs r rown off_skip_block :=
+    [(* we must first check whether the permission is O *)
+    getp r_t1 r;
+    sub_r_z r_t1 r_t1 (encodePerm O);
+    move_r r_t2 PC;
+    lea_z r_t2 4;
+    jnz r_t2 r_t1;
+    fail_end;
+    (* then we can compare the bounds *)
+    gete r_t1 r;
+    getb r_t2 rown;
+    lt_r_r r_t1 r_t1 r_t2;
+    move_r r_t2 PC;
+    lea_z r_t2 4;
+    jnz r_t2 r_t1; (* if zero we go to failure *)
+    fail_end;
+    move_r r_t2 PC;
+    lea_z r_t2 (3 + off_skip_block);
+    jmp r_t2].
+
+  Definition checkbelow_U_block_instrs r rown :=
+    [geta r_t1 r;
+    getb r_t2 rown;
+    lt_r_r r_t1 r_t1 r_t2;
+    move_r r_t2 PC;
+    lea_z r_t2 4;
+    jnz r_t2 r_t1; (* if zero we go to failure *)
+    fail_end].
+
+  Definition checkbelow_instrs r rown :=
+    branchperm_instrs r (length (checkbelow_notU_block_instrs r rown 0)) ++
+    checkbelow_notU_block_instrs r rown (length (checkbelow_U_block_instrs r rown)) ++
+    checkbelow_U_block_instrs r rown ++
+    [move_z r_t1 0;
+    move_z r_t2 0;
+    move_z r_t3 0;
+    move_z r_t4 0].
+
+  Definition checkbelow r rown a p : iProp Σ :=
+    ([∗ list] a_i;w_i ∈ a;(checkbelow_instrs r rown), a_i ↦ₐ[p] w_i)%I.
+
+  Definition isO p :=
+    match p with
+    | O => true
+    | _ => false
+    end.
+  Definition isO_word (w:Word):=
+    match w with
+    | inl _ => false
+    | inr (p,_,_,_,_) => isO p
+    end.
+
+  Lemma checkbelow_spec r rown a w p g b e a' pc_p pc_p' pc_g pc_b pc_e a_first a_last φ :
+    isCorrectPC_range pc_p pc_g pc_b pc_e a_first a_last ->
+    PermFlows pc_p pc_p' ->
+    contiguous_between a a_first a_last ->
+
+      ▷ checkbelow r rown a pc_p'
+    ∗ ▷ PC ↦ᵣ inr (pc_p,pc_g,pc_b,pc_e,a_first)
+    ∗ ▷ r ↦ᵣ w
+    ∗ ▷ rown ↦ᵣ inr (p,g,b,e,a')
+    ∗ ▷ (∃ w, r_t1 ↦ᵣ w)
+    ∗ ▷ (∃ w, r_t2 ↦ᵣ w)
+    ∗ ▷ (∃ w, r_t3 ↦ᵣ w)
+    ∗ ▷ (∃ w, r_t4 ↦ᵣ w)
+    ∗ ▷ (if (is_cap w && (canReadUpTo w <? b) && (negb (isO_word w)))%a then
+           (PC ↦ᵣ inr (pc_p,pc_g,pc_b,pc_e,a_last) ∗ checkbelow r rown a pc_p' ∗
+               r ↦ᵣ w ∗ rown ↦ᵣ inr (p,g,b,e,a') ∗ r_t1 ↦ᵣ inl 0%Z ∗ r_t2 ↦ᵣ inl 0%Z ∗ r_t3 ↦ᵣ inl 0%Z ∗ r_t4 ↦ᵣ inl 0%Z
+               -∗ WP Seq (Instr Executable) {{ φ }})
+        else φ FailedV)
+    ⊢
+    WP Seq (Instr Executable) {{ φ }}.
+  Proof.
+    iIntros (Hvpc Hfl Hcont) "(>Hprog & >HPC & >Hr & >Hrown & >Hr_t1 & >Hr_t2 & >Hr_t3 & >Hr_t4 & Hcont)".
+    iDestruct (big_sepL2_length with "Hprog") as %Hlength. simpl in *.
+    (* check block *)
+    iAssert (⌜r ≠ PC⌝)%I as %Hne.
+    { destruct (decide (r = PC)); auto; subst. iDestruct (regname_dupl_false with "HPC Hr") as %Hcontr. done. }
+    iAssert (⌜rown ≠ PC⌝)%I as %Hne'.
+    { destruct (decide (rown = PC)); auto; subst. iDestruct (regname_dupl_false with "HPC Hrown") as %Hcontr. done. }
+    iPrologue_multi "Hprog" Hcont Hvpc link.
+    iRename "Hcode" into "Hcode_first".
+    iPrologue_multi "Hprog" Hcont Hvpc link0.
+    assert ((a_first + (20%nat + 16%nat))%a = Some link0) as Hoff.
+    { clear -Hlink Hlink0. solve_addr. }
+    iApply (branchperm_spec with "[- $HPC $Hcode_first $Hr $Hr_t1 $Hr_t2 $Hr_t3 $Hr_t4]"); [apply Hvpc_code|apply Hfl|apply Hcont_code|eauto|].
+    iNext. destruct (is_cap w) eqn:Hcap;[|simpl;iFrame].
+    destruct w;inversion Hcap. destruct c,p0,p0,p0.
+    iExists _,_,_,_,_. iSplit;eauto.
+    destruct (isU p0) eqn:HU.
+    - iIntros "(HPC & Hprog_done & Hr & Hr_t1 & Hr_t2 & Hr_t3 & Hr_t4)".
+      iDestruct "Hr_t1" as (w1) "Hr_t1".
+      iDestruct "Hr_t2" as (w2) "Hr_t2".
+      iDestruct "Hr_t3" as (w3) "Hr_t3".
+      iDestruct "Hr_t4" as (w4) "Hr_t4".
+      iDestruct (big_sepL2_length with "Hprog") as %Hlength_prog. simpl in *.
+      prep_addr_list_full l_rest0 Hcont.
+      assert (pc_p ≠ E) as Hnp.
+      { eapply pc_range_not_E;eauto. }
+      pose proof (pc_range_perm _ _ _ _ _ _ _ Hvpc Hcont) as Hperms.
+      (* geta r_t1 r *)
+      iPrologue "Hprog".
+      iApply (wp_Get_success with "[$HPC $Hi $Hr $Hr_t1]");
+        [apply decode_encode_instrW_inv|auto|auto|iCorrectPC link0 a_last|iContiguous_next_a Hcont|auto..].
+      iEpilogue "(HPC & Hi & Hr & Hr_t1)";iCombine "Hi" "Hprog_done" as "Hprog_done".
+      (* getb r_t2 rown *)
+      iPrologue "Hprog".
+      iApply (wp_Get_success with "[$HPC $Hi $Hrown $Hr_t2]");
+        [apply decode_encode_instrW_inv|auto|auto|iCorrectPC link0 a_last|iContiguous_next_a Hcont|auto..].
+      iEpilogue "(HPC & Hi & Hrown & Hr_t2)";iCombine "Hi" "Hprog_done" as "Hprog_done".
+      (* lt r_t1 r_t1 r_t2 *)
+      iPrologue "Hprog".
+      iApply (wp_add_sub_lt_success_dst_r with "[$HPC $Hi $Hr_t2 $Hr_t1]");
+        [apply decode_encode_instrW_inv|eauto|iContiguous_next_a Hcont|auto|iCorrectPC link0 a_last|auto..].
+      iEpilogue "(HPC & Hi & Hr_t2 & Hr_t1)";iCombine "Hi" "Hprog_done" as "Hprog_done".
+      (* move r_t2 PC *)
+      iPrologue "Hprog".
+      iApply (wp_move_success_reg_fromPC with "[$HPC $Hi $Hr_t2]");
+        [apply decode_encode_instrW_inv|auto|iCorrectPC link0 a_last|iContiguous_next_a Hcont|auto..].
+      iEpilogue "(HPC & Hi & Hr_t2)";iCombine "Hi" "Hprog_done" as "Hprog_done".
+      (* lea r_t2 4 *)
+      assert (a5 + 4 = Some a9)%a as Hlea.
+      { apply contiguous_between_incr_addr_middle with (i:=3) (j:=4) (ai:=a5) (aj:=a9) in Hcont;auto. }
+      iPrologue "Hprog".
+      iApply (wp_lea_success_z with "[$HPC $Hi $Hr_t2]");
+        [apply decode_encode_instrW_inv|auto|iCorrectPC link0 a_last|iContiguous_next_a Hcont|apply Hlea|auto..].
+      { destruct Hperms as [-> | [-> | ->] ]; auto. }
+      iEpilogue "(HPC & Hi & Hr_t2)";iCombine "Hi" "Hprog_done" as "Hprog_done".
+      (* jnz r_t1 r_t2 *)
+      iPrologue "Hprog". iSimpl in "Hr_t1".
+      destruct (decide ((Z.b2z (a0 <? b)%Z) = 0)).
+      + rewrite e0.
+        iApply (wp_jnz_success_next with "[$HPC $Hi $Hr_t2 $Hr_t1]");
+          [apply decode_encode_instrW_inv|auto|iCorrectPC link0 a_last|iContiguous_next_a Hcont|auto..].
+        iEpilogue "(HPC & Hi & Hr_t2 & Hr_t1)";iCombine "Hi" "Hprog_done" as "Hprog_done".
+        (* fail *)
+        iPrologue "Hprog".
+        iApply (wp_fail with "[$HPC $Hi]");
+          [apply decode_encode_instrW_inv|auto|iCorrectPC link0 a_last|..].
+        iEpilogue "(HPC & Hi)". iApply wp_value.
+        assert (match p0 with
+                | O => 0
+                | URW | URWL | URWX | URWLX => a0
+                | _ => a1
+                end = a0)%a as ->.
+        { destruct p0;auto;inversion HU. }
+        destruct (a0 <? b)%Z eqn:Hbool;[inversion e0|].
+        assert (a0 <? b = false)%a as ->;[clear -Hbool;solve_addr|].
+        iFrame.
+      + iApply (wp_jnz_success_jmp with "[$HPC $Hi $Hr_t2 $Hr_t1]");
+          [apply decode_encode_instrW_inv|auto|iCorrectPC link0 a_last|auto..].
+        { intros Hcontr; inversion Hcontr. done. }
+        iEpilogue "(HPC & Hi & Hr_t2 &  Hr_t1)";iCombine "Hi" "Hprog_done" as "Hprog_done".
+        iDestruct "Hprog" as "[Hi Hprog]"; iCombine "Hi" "Hprog_done" as "Hprog_done".
+        (* move r_t1 0 *)
+        rewrite updatePcPerm_cap_non_E //.
+        iPrologue "Hprog".
+        iApply (wp_move_success_z with "[$HPC $Hi $Hr_t1]");
+          [apply decode_encode_instrW_inv|auto|iCorrectPC link0 a_last|iContiguous_next_a Hcont|].
+        iEpilogue "(HPC & Hi & Hr_t1)";iCombine "Hi" "Hprog_done" as "Hprog_done".
+        (* move r_t2 0 *)
+        iPrologue "Hprog".
+        iApply (wp_move_success_z with "[$HPC $Hi $Hr_t2]");
+          [apply decode_encode_instrW_inv|auto|iCorrectPC link0 a_last|iContiguous_next_a Hcont|].
+        iEpilogue "(HPC & Hi & Hr_t2)";iCombine "Hi" "Hprog_done" as "Hprog_done".
+        (* move r_t3 0 *)
+        iPrologue "Hprog".
+        iApply (wp_move_success_z with "[$HPC $Hi $Hr_t3]");
+          [apply decode_encode_instrW_inv|auto|iCorrectPC link0 a_last|iContiguous_next_a Hcont|].
+        iEpilogue "(HPC & Hi & Hr_t3)";iCombine "Hi" "Hprog_done" as "Hprog_done".
+        (* move r_t4 0 *)
+        iPrologue "Hprog".
+        iApply (wp_move_success_z with "[$HPC $Hi $Hr_t4]");
+          [apply decode_encode_instrW_inv|auto|iCorrectPC link0 a_last|eapply contiguous_between_last;[apply Hcont|auto]|].
+        iEpilogue "(HPC & Hi & Hr_t4)";iCombine "Hi" "Hprog_done" as "Hprog_done".
+        (* cont *)
+        assert (match p0 with
+                | O => 0
+                | URW | URWL | URWX | URWLX => a0
+                | _ => a1
+                end = a0)%a as ->.
+        { destruct p0;auto;inversion HU. }
+        destruct (a0 <? b)%Z eqn:Hbool;[|contradiction].
+        assert (a0 <? b = true)%a as ->;[clear -Hbool;solve_addr|].
+        assert (negb (isO p0) = true) as ->;[destruct p0;auto|].
+        iApply "Hcont". iFrame "HPC Hr Hr_t1 Hr_t2 Hr_t3 Hr_t4 Hrown Hcode".
+        iDestruct "Hprog_done" as "($&$&$&$&$&$&$&$&$&$&$&?)". iFrame.
+    - iIntros "(HPC & Hprog_done & Hr & Hr_t1 & Hr_t2 & Hr_t3 & Hr_t4)".
+      iDestruct "Hr_t1" as (w1) "Hr_t1".
+      iDestruct "Hr_t2" as (w2) "Hr_t2".
+      iDestruct "Hr_t3" as (w3) "Hr_t3".
+      iDestruct "Hr_t4" as (w4) "Hr_t4".
+      iRename "Hprog" into "Hskipped". iRename "Hcode" into "Hprog".
+      rename link0 into linkskipped. rename link into link0.
+      rename Hcont into Hcont_skipped. rename Hcont_code0 into Hcont.
+      rename Hvpc into Hvpc_skipped. rename Hvpc_code0 into Hvpc.
+      iDestruct (big_sepL2_length with "Hprog") as %Hlength_prog. simpl in *.
+      prep_addr_list_full l_code0 Hcont.
+      assert (pc_p ≠ E) as Hnp.
+      { eapply pc_range_not_E;[apply Hvpc|]. eauto. }
+      pose proof (pc_range_perm _ _ _ _ _ _ _ Hvpc Hcont) as Hperms.
+      (* getp r_t1 r *)
+      iPrologue "Hprog".
+      iApply (wp_Get_success with "[$HPC $Hi $Hr $Hr_t1]");
+        [apply decode_encode_instrW_inv|auto|auto|iCorrectPC link0 linkskipped|iContiguous_next_a Hcont|auto..].
+      iEpilogue "(HPC & Hi & Hr & Hr_t1)";iCombine "Hi" "Hprog_done" as "Hprog_done".
+      iSimpl in "Hr_t1".
+      (* sub r_t1 r_t1 O *)
+      iPrologue "Hprog".
+      iApply (wp_add_sub_lt_success_dst_z with "[$HPC $Hi $Hr_t1]");
+        [apply decode_encode_instrW_inv|eauto|iContiguous_next_a Hcont|auto|iCorrectPC link0 linkskipped|..].
+      iEpilogue "(HPC & Hi & Hr_t1)";iCombine "Hi" "Hprog_done" as "Hprog_done".
+      (* move r_t2 PC *)
+      iPrologue "Hprog".
+      iApply (wp_move_success_reg_fromPC with "[$HPC $Hi $Hr_t2]");
+        [apply decode_encode_instrW_inv|auto|iCorrectPC link0 linkskipped|iContiguous_next_a Hcont|auto..].
+      iEpilogue "(HPC & Hi & Hr_t2)";iCombine "Hi" "Hprog_done" as "Hprog_done".
+      (* lea r_t2 4 *)
+      assert (a4 + 4 = Some a8)%a as Hlea.
+      { apply contiguous_between_incr_addr_middle with (i:=2) (j:=4) (ai:=a4) (aj:=a8) in Hcont;auto. }
+      iPrologue "Hprog".
+      iApply (wp_lea_success_z with "[$HPC $Hi $Hr_t2]");
+        [apply decode_encode_instrW_inv|auto|iCorrectPC link0 linkskipped|iContiguous_next_a Hcont|apply Hlea|auto..].
+      { destruct Hperms as [-> | [-> | ->] ]; auto. }
+      iEpilogue "(HPC & Hi & Hr_t2)";iCombine "Hi" "Hprog_done" as "Hprog_done".
+      (* jnz r_t2 r_t1 *)
+      iPrologue "Hprog". iSimpl in "Hr_t1".
+      destruct (decide (encodePerm p0 - encodePerm O = 0)%Z).
+      { (* the permission is O, we can simply fail since jumping to an O cap will fail anyways *)
+        rewrite e0.
+        iApply (wp_jnz_success_next with "[$HPC $Hi $Hr_t2 $Hr_t1]");
+          [apply decode_encode_instrW_inv|auto|iCorrectPC link0 linkskipped|iContiguous_next_a Hcont|auto..].
+        iEpilogue "(HPC & Hi & Hr_t2 & Hr_t1)";iCombine "Hi" "Hprog_done" as "Hprog_done".
+        (* fail *)
+        iPrologue "Hprog".
+        iApply (wp_fail with "[$HPC $Hi]");
+          [apply decode_encode_instrW_inv|auto|iCorrectPC link0 linkskipped|..].
+        iEpilogue "(HPC & Hi)". iApply wp_value.
+        assert (p0 = O) as ->;[apply encodePerm_inj;lia|]. rewrite andb_false_r. iFrame.
+      }
+      (* now we know that p0 is not O *)
+      assert (p0 ≠ O) as HnO;[intros Hcontr;subst;lia|].
+      iApply (wp_jnz_success_jmp with "[$HPC $Hi $Hr_t2 $Hr_t1]");
+        [apply decode_encode_instrW_inv|auto|iCorrectPC link0 linkskipped|auto..].
+      { intros Hcontr; inversion Hcontr. done. }
+      iEpilogue "(HPC & Hi & Hr_t2 &  Hr_t1)";iCombine "Hi" "Hprog_done" as "Hprog_done".
+      iDestruct "Hprog" as "[Hi Hprog]"; iCombine "Hi" "Hprog_done" as "Hprog_done".
+      (* gete r_t1 r *)
+      rewrite updatePcPerm_cap_non_E //.
+      iPrologue "Hprog".
+      iApply (wp_Get_success with "[$HPC $Hi $Hr $Hr_t1]");
+        [apply decode_encode_instrW_inv|auto|auto|iCorrectPC link0 linkskipped|iContiguous_next_a Hcont|auto..].
+      iEpilogue "(HPC & Hi & Hr & Hr_t1)";iCombine "Hi" "Hprog_done" as "Hprog_done".
+      (* getb r_t2 rown *)
+      iPrologue "Hprog".
+      iApply (wp_Get_success with "[$HPC $Hi $Hrown $Hr_t2]");
+        [apply decode_encode_instrW_inv|auto|auto|iCorrectPC link0 linkskipped|iContiguous_next_a Hcont|auto..].
+      iEpilogue "(HPC & Hi & Hrown & Hr_t2)";iCombine "Hi" "Hprog_done" as "Hprog_done".
+      (* lt r_t1 r_t1 r_t2 *)
+      iPrologue "Hprog".
+      iApply (wp_add_sub_lt_success_dst_r with "[$HPC $Hi $Hr_t2 $Hr_t1]");
+        [apply decode_encode_instrW_inv|eauto|iContiguous_next_a Hcont|auto|iCorrectPC link0 linkskipped|auto..].
+      iEpilogue "(HPC & Hi & Hr_t2 & Hr_t1)";iCombine "Hi" "Hprog_done" as "Hprog_done".
+      (* move r_t2 PC *)
+      iPrologue "Hprog".
+      iApply (wp_move_success_reg_fromPC with "[$HPC $Hi $Hr_t2]");
+        [apply decode_encode_instrW_inv|auto|iCorrectPC link0 linkskipped|iContiguous_next_a Hcont|auto..].
+      iEpilogue "(HPC & Hi & Hr_t2)";iCombine "Hi" "Hprog_done" as "Hprog_done".
+      (* lea r_t2 4 *)
+      assert (a11 + 4 = Some a15)%a as Hlea'.
+      { apply contiguous_between_incr_addr_middle with (i:=9) (j:=4) (ai:=a11) (aj:=a15) in Hcont;auto. }
+      iPrologue "Hprog".
+      iApply (wp_lea_success_z with "[$HPC $Hi $Hr_t2]");
+        [apply decode_encode_instrW_inv|auto|iCorrectPC link0 linkskipped|iContiguous_next_a Hcont|apply Hlea'|auto..].
+      { destruct Hperms as [-> | [-> | ->] ]; auto. }
+      iEpilogue "(HPC & Hi & Hr_t2)";iCombine "Hi" "Hprog_done" as "Hprog_done".
+      (* jnz r_t1 r_t2 *)
+      iPrologue "Hprog". iSimpl in "Hr_t1".
+      destruct (decide ((Z.b2z (a1 <? b)%Z) = 0)).
+      + rewrite e0.
+        iApply (wp_jnz_success_next with "[$HPC $Hi $Hr_t2 $Hr_t1]");
+          [apply decode_encode_instrW_inv|auto|iCorrectPC link0 linkskipped|iContiguous_next_a Hcont|auto..].
+        iEpilogue "(HPC & Hi & Hr_t2 & Hr_t1)";iCombine "Hi" "Hprog_done" as "Hprog_done".
+        (* fail *)
+        iPrologue "Hprog".
+        iApply (wp_fail with "[$HPC $Hi]");
+          [apply decode_encode_instrW_inv|auto|iCorrectPC link0 linkskipped|..].
+        iEpilogue "(HPC & Hi)". iApply wp_value.
+        assert (match p0 with
+                | O => 0
+                | URW | URWL | URWX | URWLX => a0
+                | _ => a1
+                end = a1)%a as ->.
+        { destruct p0;auto;inversion HU. contradiction. }
+        destruct (a1 <? b)%Z eqn:Hbool;[inversion e0|].
+        assert (a1 <? b = false)%a as ->;[clear -Hbool;solve_addr|].
+        iFrame.
+      + iApply (wp_jnz_success_jmp with "[$HPC $Hi $Hr_t2 $Hr_t1]");
+          [apply decode_encode_instrW_inv|auto|iCorrectPC link0 linkskipped|auto..].
+        { intros Hcontr; inversion Hcontr. done. }
+        iEpilogue "(HPC & Hi & Hr_t2 &  Hr_t1)";iCombine "Hi" "Hprog_done" as "Hprog_done".
+        iDestruct "Hprog" as "[Hi Hprog]"; iCombine "Hi" "Hprog_done" as "Hprog_done".
+        (* move r_t2 PC *)
+        iPrologue "Hprog". rewrite updatePcPerm_cap_non_E //.
+        iApply (wp_move_success_reg_fromPC with "[$HPC $Hi $Hr_t2]");
+          [apply decode_encode_instrW_inv|auto|iCorrectPC link0 linkskipped|iContiguous_next_a Hcont|auto..].
+        iEpilogue "(HPC & Hi & Hr_t2)";iCombine "Hi" "Hprog_done" as "Hprog_done".
+        (* lea r_t2 10 *)
+        iDestruct (big_sepL2_length with "Hskipped") as %Hlength_skipped. simpl in *.
+        prep_addr_list_full l_rest0 Hcont_skipped.
+        assert (a15 + 10 = Some a24)%a as Hlea''.
+        { apply contiguous_between_incr_addr_middle with (i:=0) (j:=7) (ai:=linkskipped) (aj:=a24) in Hcont_skipped;auto.
+          apply contiguous_between_middle_to_end with (i:=13) (ai:=a15) (k:=3) in Hcont;auto.
+          clear -Hcont Hcont_skipped. solve_addr. }
+        iPrologue "Hprog".
+        iApply (wp_lea_success_z with "[$HPC $Hi $Hr_t2]");
+          [apply decode_encode_instrW_inv|auto|iCorrectPC link0 linkskipped|iContiguous_next_a Hcont|apply Hlea''|auto..].
+        { destruct Hperms as [-> | [-> | ->] ]; auto. }
+        iEpilogue "(HPC & Hi & Hr_t2)";iCombine "Hi" "Hprog_done" as "Hprog_done".
+        (* jmp r_t2 *)
+        iPrologue "Hprog".
+        iApply (wp_jmp_success with "[$HPC $Hi $Hr_t2]");
+          [apply decode_encode_instrW_inv|auto|iCorrectPC link0 linkskipped|..].
+        iEpilogue "(HPC & Hi & Hr_t2)";iCombine "Hi" "Hprog_done" as "Hprog_done".
+        rewrite updatePcPerm_cap_non_E //.
+        do 7 (iDestruct "Hskipped" as "[Hi Hskipped]"; iCombine "Hi" "Hprog_done" as "Hprog_done").
+        (* move r_t1 0 *)
+        iClear "Hprog". iRename "Hskipped" into "Hprog".
+        iPrologue "Hprog".
+        iApply (wp_move_success_z with "[$HPC $Hi $Hr_t1]");
+          [apply decode_encode_instrW_inv|auto|iCorrectPC linkskipped a_last|iContiguous_next_a Hcont_skipped|].
+        iEpilogue "(HPC & Hi & Hr_t1)";iCombine "Hi" "Hprog_done" as "Hprog_done".
+        (* move r_t2 0 *)
+        iPrologue "Hprog".
+        iApply (wp_move_success_z with "[$HPC $Hi $Hr_t2]");
+          [apply decode_encode_instrW_inv|auto|iCorrectPC linkskipped a_last|iContiguous_next_a Hcont_skipped|].
+        iEpilogue "(HPC & Hi & Hr_t2)";iCombine "Hi" "Hprog_done" as "Hprog_done".
+        (* move r_t3 0 *)
+        iPrologue "Hprog".
+        iApply (wp_move_success_z with "[$HPC $Hi $Hr_t3]");
+          [apply decode_encode_instrW_inv|auto|iCorrectPC linkskipped a_last|iContiguous_next_a Hcont_skipped|].
+        iEpilogue "(HPC & Hi & Hr_t3)";iCombine "Hi" "Hprog_done" as "Hprog_done".
+        (* move r_t4 0 *)
+        iPrologue "Hprog".
+        iApply (wp_move_success_z with "[$HPC $Hi $Hr_t4]");
+          [apply decode_encode_instrW_inv|auto|iCorrectPC linkskipped a_last|eapply contiguous_between_last;[apply Hcont_skipped|auto]|].
+        iEpilogue "(HPC & Hi & Hr_t4)";iCombine "Hi" "Hprog_done" as "Hprog_done".
+        (* cont *)
+        assert (match p0 with
+                | O => 0
+                | URW | URWL | URWX | URWLX => a0
+                | _ => a1
+                end = a1)%a as ->.
+        { destruct p0;auto;inversion HU. contradiction. }
+        destruct (a1 <? b)%Z eqn:Hbool;[|contradiction].
+        assert (a1 <? b = true)%a as ->;[clear -Hbool;solve_addr|].
+        assert (negb (isO p0) = true) as ->;[destruct p0;auto|].
+        iApply "Hcont". iFrame "HPC Hr Hr_t1 Hr_t2 Hr_t3 Hr_t4 Hrown".
+        iDestruct "Hprog_done" as "($&$&$&$&$&$&$&$&$&$&$&$&$&$&$&$&$&$&$&$&$&$&$&$&$&$&$&$)".
+        done.
+  Qed.
+
+
+End stack_macros.
