theories/examples/macros/macros.v
@@ -1,0 +1,5 @@
+From cap_machine Require Export
+     addr_reg_sample region_macros contiguous
+     stack_macros_helpers.
+
+From cap_machine Require Export malloc req push_pop prepstack rclear checkbelow.
