theories/examples/macros/malloc.v
@@ -1,0 +1,765 @@
+From iris.algebra Require Import frac.
+From iris.proofmode Require Import tactics.
+From cap_machine Require Import rules logrel addr_reg_sample fundamental multiple_updates.
+From cap_machine.examples Require Import contiguous stack_macros_helpers.
+From iris.base_logic Require Export na_invariants.
+
+(* A toy malloc implementation *)
+
+(* The routine is initially provided a capability to a contiguous range of
+   memory. It implements a bump-pointer allocator, where all memory before the
+   pointer of the capability has been allocated, and all memory after is free.
+   Allocating corresponds to increasing the pointer and returning the
+   corresponding sub-slice.
+
+   There is no free: when all the available memory has been allocated, the
+   routine cannot allocate new memory and will fail instead.
+
+   This is obviously not very realistic, but is good enough for our simple case
+   studies. *)
+
+Section SimpleMalloc.
+  Context {Σ:gFunctors} {memg:memG Σ} {regg:regG Σ}
+          {stsg : STSG Addr region_type Σ} {heapg : heapG Σ}
+          `{MonRef: MonRefG (leibnizO _) CapR_rtc Σ} {nainv: logrel_na_invs Σ}
+          `{MP: MachineParameters}.
+
+  Definition malloc_subroutine_instrs' (offset: Z) :=
+    [lt_z_r r_t3 0 r_t1;
+     move_r r_t2 PC;
+     lea_z r_t2 4; 
+     jnz r_t2 r_t3;
+     fail_end;
+     move_r r_t2 PC;
+     lea_z r_t2 offset;
+     load_r r_t2 r_t2;
+     geta r_t3 r_t2;
+     lea_r r_t2 r_t1;
+     geta r_t1 r_t2;
+     move_r r_t4 r_t2;
+     subseg_r_r r_t4 r_t3 r_t1;
+     sub_r_r r_t3 r_t3 r_t1;
+     lea_r r_t4 r_t3;
+     move_r r_t3 r_t2;
+     sub_z_r r_t1 0%Z r_t1;
+     lea_r r_t3 r_t1;
+     getb r_t1 r_t3;
+     lea_r r_t3 r_t1;
+     store_r r_t3 r_t2;
+     move_r r_t1 r_t4;
+     move_z r_t2 0%Z;
+     move_z r_t3 0%Z;
+     move_z r_t4 0%Z;
+     jmp r_t0].
+
+  Definition malloc_subroutine_instrs_length : Z :=
+    Eval cbv in (length (malloc_subroutine_instrs' 0%Z)).
+
+  Definition malloc_subroutine_instrs :=
+    malloc_subroutine_instrs' (malloc_subroutine_instrs_length - 5).
+
+  Ltac iPrologue_pre :=
+    match goal with
+    | Hlen : length ?a = ?n |- _ =>
+      let a' := fresh "a" in
+      destruct a as [| a' a]; inversion Hlen; simpl
+    end.
+
+  Ltac iPrologue prog :=
+    (try iPrologue_pre);
+    iDestruct prog as "[Hi Hprog]";
+    iApply (wp_bind (fill [SeqCtx])).
+
+  Ltac iEpilogue prog :=
+    iNext; iIntros prog; iSimpl;
+    iApply wp_pure_step_later;auto;iNext.
+
+  Ltac iCorrectPC i j :=
+    eapply isCorrectPC_contiguous_range with (a0 := i) (an := j); eauto; [];
+    cbn; solve [ repeat constructor ].
+
+  Ltac iContiguous_next Ha index :=
+    apply contiguous_of_contiguous_between in Ha;
+    generalize (contiguous_spec _ Ha index); auto.
+
+  Definition malloc_inv (b e : Addr) : iProp Σ :=
+    (∃ b_m a_m,
+       [[b, b_m]] ↦ₐ[RX] [[ malloc_subroutine_instrs ]]
+     ∗ b_m ↦ₐ[RWX] (inr (RWX, Global, b_m, e, a_m))
+     ∗ [[a_m, e]] ↦ₐ[RWX] [[ region_addrs_zeroes a_m e ]]
+     ∗ ⌜(b_m < a_m)%a ∧ (a_m <= e)%a⌝
+    )%I.
+
+
+  (* TODO: move this to the rules_AddSubLt.v file. *)
+  Lemma wp_AddSubLt_fail E ins dst n1 r2 w wdst cap pc_p pc_p' pc_g pc_b pc_e pc_a :
+    decodeInstrW w = ins
+    → PermFlows pc_p pc_p'
+    → is_AddSubLt ins dst (inl n1) (inr r2)
+      (* → (pc_a + 1)%a = Some pc_a' *)
+        → isCorrectPC (inr (pc_p, pc_g, pc_b, pc_e, pc_a))
+          → {{{ PC ↦ᵣ inr (pc_p, pc_g, pc_b, pc_e, pc_a) ∗ pc_a ↦ₐ[pc_p'] w ∗ dst ↦ᵣ wdst ∗ r2 ↦ᵣ inr cap }}}
+              Instr Executable
+            @ E
+      {{{ RET FailedV; True }}}.
+  Proof.
+    iIntros (Hdecode Hperm Hinstr Hvpc φ) "(HPC & Hpc_a & Hdst & Hr2) Hφ".
+    iDestruct (rules_base.map_of_regs_3 with "HPC Hdst Hr2") as "[Hmap (%&%&%)]".
+    iApply (wp_AddSubLt with "[$Hmap Hpc_a]"); eauto; simplify_map_eq; eauto.
+      by erewrite regs_of_is_AddSubLt; eauto; rewrite !dom_insert; set_solver+.
+    iNext. iIntros (regs' retv) "(#Hspec & Hpc_a & Hmap)". iDestruct "Hspec" as %Hspec.
+    destruct Hspec as [* Hsucc |].
+    { (* Success (contradiction) *) simplify_map_eq. }
+    { (* Failure, done *) by iApply "Hφ". }
+  Qed.
+
+
+  Lemma simple_malloc_subroutine_spec (wsize: Word) (cont: Word) b e rmap N E φ :
+    dom (gset RegName) rmap = all_registers_s ∖ {[ PC; r_t0; r_t1 ]} →
+    (* (size > 0)%Z → *)
+    ↑N ⊆ E →
+    (  na_inv logrel_nais N (malloc_inv b e)
+     ∗ na_own logrel_nais E
+     ∗ ([∗ map] r↦w ∈ rmap, r ↦ᵣ w)
+     ∗ r_t0 ↦ᵣ cont
+     ∗ PC ↦ᵣ inr (RX, Global, b, e, b)
+     ∗ r_t1 ↦ᵣ wsize
+     ∗ ▷ ((na_own logrel_nais E
+          ∗ [∗ map] r↦w ∈ <[r_t2 := inl 0%Z]>
+                         (<[r_t3 := inl 0%Z]>
+                         (<[r_t4 := inl 0%Z]>
+                          rmap)), r ↦ᵣ w)
+          ∗ r_t0 ↦ᵣ cont
+          ∗ PC ↦ᵣ updatePcPerm cont
+          ∗ (∃ (ba ea : Addr) (size : Z),
+                ⌜wsize = inl size⌝
+            ∗ ⌜(b <= ba ∧ ea ≤ e)%Z⌝
+            ∗ ⌜(size > 0)%Z⌝
+            ∗ ⌜(ba + size)%a = Some ea⌝
+            ∗ r_t1 ↦ᵣ inr (RWX, Global, ba, ea, ba)
+            ∗ [[ba, ea]] ↦ₐ[RWX] [[region_addrs_zeroes ba ea]])
+          -∗ WP Seq (Instr Executable) {{ φ }}))
+    ⊢ WP Seq (Instr Executable) {{ λ v, φ v ∨ ⌜v = FailedV⌝ }}%I.
+  Proof.
+    iIntros (Hrmap_dom (* Hsize *) HN) "(#Hinv & Hna & Hrmap & Hr0 & HPC & Hr1 & Hφ)".
+    iMod (na_inv_acc with "Hinv Hna") as "(>Hmalloc & Hna & Hinv_close)"; auto.
+    rewrite /malloc_inv.
+    iDestruct "Hmalloc" as (b_m a_m) "(Hprog & Hmemptr & Hmem & Hbounds)".
+    iDestruct "Hbounds" as %[Hbm_am Ham_e].
+    (* Get some registers *)
+    assert (is_Some (rmap !! r_t2)) as [r2w Hr2w].
+    { rewrite elem_of_gmap_dom Hrmap_dom. set_solver. }
+    assert (is_Some (rmap !! r_t3)) as [r3w Hr3w].
+    { rewrite elem_of_gmap_dom Hrmap_dom. set_solver. }
+    assert (is_Some (rmap !! r_t4)) as [r4w Hr4w].
+    { rewrite elem_of_gmap_dom Hrmap_dom. set_solver. }
+    iDestruct (big_sepM_delete _ _ r_t2 with "Hrmap") as "[Hr2 Hrmap]".
+      eassumption.
+    iDestruct (big_sepM_delete _ _ r_t3 with "Hrmap") as "[Hr3 Hrmap]".
+      by rewrite lookup_delete_ne //.
+    iDestruct (big_sepM_delete _ _ r_t4 with "Hrmap") as "[Hr4 Hrmap]".
+      by rewrite !lookup_delete_ne //.
+      
+    rewrite /(region_mapsto b b_m).
+    set ai := region_addrs b b_m.
+    assert (Hai: region_addrs b b_m = ai) by reflexivity.
+    iDestruct (big_sepL2_length with "Hprog") as %Hprog_len.
+    cbn in Hprog_len.
+    assert ((b + malloc_subroutine_instrs_length)%a = Some b_m) as Hb_bm.
+    { rewrite /malloc_subroutine_instrs_length.
+      rewrite region_addrs_length /region_size in Hprog_len. solve_addr. }
+    assert (contiguous_between ai b b_m) as Hcont.
+    { apply contiguous_between_of_region_addrs; eauto.
+      rewrite /malloc_subroutine_instrs_length in Hb_bm. solve_addr. }
+
+    assert (HPC: ∀ a, a ∈ ai → isCorrectPC (inr (RX, Global, b, e, a))).
+    { intros a Ha.
+      pose proof (contiguous_between_middle_bounds' _ _ _ _ Hcont Ha) as [? ?].
+      constructor; eauto. solve_addr. }
+
+    (* lt r_t3 0 r_t1 *)
+    destruct ai as [|a l];[inversion Hprog_len|].
+    destruct l as [|? l];[inversion Hprog_len|].
+    pose proof (contiguous_between_cons_inv_first _ _ _ _ Hcont) as ->.
+    iPrologue "Hprog".
+    destruct (wsize) as [size|]. 
+    2: { iApply (wp_AddSubLt_fail with "[$HPC $Hi $Hr3 $Hr1]");
+         [apply decode_encode_instrW_inv|apply PermFlows_refl|right;right;eauto|..].
+         { apply HPC; repeat constructor. }
+         iEpilogue "_". iApply wp_value. by iRight.
+    }
+    iApply (wp_add_sub_lt_success_z_r with "[$HPC $Hi $Hr3 $Hr1]");
+      [apply decode_encode_instrW_inv|right;right;eauto|iContiguous_next Hcont 0|done|..]. 
+    { apply HPC; repeat constructor. }
+    iEpilogue "(HPC & Hprog_done & Hr1 & Hr3)".
+    (* move r_t2 PC *)
+    destruct l as [|? l];[inversion Hprog_len|].    
+    iPrologue "Hprog".
+    iApply (wp_move_success_reg_fromPC with "[$HPC $Hi $Hr2]");
+      [apply decode_encode_instrW_inv|done| |iContiguous_next Hcont 1|auto|..].
+    { apply HPC; repeat constructor. }
+    iEpilogue "(HPC & Hi & Hr2)". iCombine "Hi" "Hprog_done" as "Hprog_done".
+    (* lea r_t2 4 *)
+    do 3 (destruct l as [|? l];[inversion Hprog_len|]). 
+    assert (a0 + 4 = Some a3)%a as Hlea1.
+    { apply contiguous_between_incr_addr_middle with (i:=1) (j:=4) (ai:=a0) (aj:=a3) in Hcont;auto. }
+    iPrologue "Hprog".
+    iApply (wp_lea_success_z with "[$HPC $Hi $Hr2]");
+      [apply decode_encode_instrW_inv|done| |iContiguous_next Hcont 2|try done..].
+    { apply HPC; repeat constructor. }
+    iEpilogue "(HPC & Hi & Hr2)". iCombine "Hi" "Hprog_done" as "Hprog_done".
+
+    (* we need do destruct on the cases for the size *)
+    destruct (decide (0 < size)%Z) as [Hsize | Hsize]. 
+    2: {
+      (* the program will not jump, and go to the fail instruction *)
+      (* jnz  r_t2 r_t3 *)
+      assert (rules_AddSubLt.denote (Lt r_t3 (inl 0%Z) (inr r_t1)) 0 size = 0) as ->.
+      { simpl. clear -Hsize. apply Z.ltb_nlt in Hsize. rewrite Hsize. auto. }
+      iPrologue "Hprog".
+      iApply (wp_jnz_success_next with "[$HPC $Hi $Hr2 $Hr3]");
+        [apply decode_encode_instrW_inv|done| |iContiguous_next Hcont 3|..]. 
+      { apply HPC; repeat constructor. }
+      iEpilogue "(HPC & Hi & Hr2 & Hr3)". iCombine "Hi" "Hprog_done" as "Hprog_done".
+      (* fail *)
+      iPrologue "Hprog".
+      iApply (wp_fail with "[$HPC $Hi]");
+        [apply decode_encode_instrW_inv|done|..].
+      { apply HPC; repeat constructor. }
+      iEpilogue "_". iApply wp_value. by iRight.
+    }
+
+    (* otherwise we continue malloc *)
+    iPrologue "Hprog".
+    assert (rules_AddSubLt.denote (Lt r_t3 (inl 0%Z) (inr r_t1)) 0 size = 1) as ->.
+    { simpl. clear -Hsize. apply Z.ltb_lt in Hsize. rewrite Hsize. auto. }
+    iApply (wp_jnz_success_jmp with "[$HPC $Hi $Hr2 $Hr3]");
+        [apply decode_encode_instrW_inv|done| |iContiguous_next Hcont 3|..]. 
+    { apply HPC; repeat constructor. }
+    iEpilogue "(HPC & Hi & Hr2 & Hr3)". iCombine "Hi" "Hprog_done" as "Hprog_done".
+    
+    (* move r_t2 PC *)
+    destruct l as [|? l];[inversion Hprog_len|].
+    iPrologue "Hprog". iCombine "Hi" "Hprog_done" as "Hprog_done".
+    iDestruct "Hprog" as "[Hi Hprog]". 
+    iApply (wp_move_success_reg_fromPC with "[$HPC $Hi $Hr2]");
+      [apply decode_encode_instrW_inv|done| |iContiguous_next Hcont 5|auto..].
+    { apply HPC; repeat constructor. }
+    iEpilogue "(HPC & Hi & Hr2)".
+    (* lea r_t2 malloc_instrs_length *)
+    destruct l as [|? l];[inversion Hprog_len|]. iCombine "Hi" "Hprog_done" as "Hprog_done".
+    iPrologue "Hprog".
+    assert ((a3 + (malloc_subroutine_instrs_length - 5))%a = Some b_m) as Hlea.
+    { assert (b + 5 = Some a3)%a. apply contiguous_between_incr_addr with (i:=5) (ai:=a3) in Hcont;auto.
+      clear -H Hb_bm. solve_addr. }
+    iApply (wp_lea_success_z with "[$HPC $Hi $Hr2]");
+      [apply decode_encode_instrW_inv|done| |iContiguous_next Hcont 6|apply Hlea|try done..].
+    { apply HPC; repeat constructor. }
+    iEpilogue "(HPC & Hi & Hr2)". iCombine "Hi" "Hprog_done" as "Hprog_done".
+    (* load r_t2 r_t2 *)
+    destruct l as [|? l];[inversion Hprog_len|].
+    iPrologue "Hprog".
+    (* FIXME *)
+    assert ((b_m =? a5)%a = false) as Hbm_a.
+    { apply Z.eqb_neq. intro.
+      pose proof (contiguous_between_middle_bounds _ 7 a5 _ _ Hcont eq_refl) as [? ?].
+      solve_addr. }
+    iApply (wp_load_success_same with "[$HPC $Hi $Hr2 Hmemptr]");
+      [auto(*FIXME*)|apply decode_encode_instrW_inv|done| |split;try done
+       |iContiguous_next Hcont 7|..].
+    { apply HPC; repeat constructor. }
+    { apply le_addr_withinBounds.
+      - generalize (contiguous_between_length _ _ _ Hcont). cbn.
+        clear; solve_addr.
+      - revert Hbm_am Ham_e; solve_addr. }
+    { rewrite Hbm_a; iFrame. auto. }
+    rewrite Hbm_a. iEpilogue "(HPC & Hr2 & Hi & Hmemptr)".
+    iCombine "Hi" "Hprog_done" as "Hprog_done".
+    (* geta r_t3 r_t2 *)
+    destruct l as [|? l];[inversion Hprog_len|].
+    iPrologue "Hprog".
+    iApply (wp_Get_success with "[$HPC $Hi $Hr3 $Hr2]");
+      [apply decode_encode_instrW_inv|done|done| |iContiguous_next Hcont 8|auto..].
+    { apply HPC; repeat constructor. }
+    iEpilogue "(HPC & Hi & Hr2 & Hr3)". iCombine "Hi" "Hprog_done" as "Hprog_done".
+    cbn [rules_Get.denote].
+    (* lea_r r_t2 r_t1 *)
+    destruct l as [|? l];[inversion Hprog_len|].
+    iPrologue "Hprog".
+    destruct (a_m + size)%a as [a_m'|] eqn:Ha_m'; cycle 1.
+    { iAssert ([∗ map] k↦x ∈ (∅:gmap RegName Word), k ↦ᵣ x)%I as "Hregs".
+        by rewrite big_sepM_empty.
+      iDestruct (big_sepM_insert with "[$Hregs $HPC]") as "Hregs'".
+        by apply lookup_empty.
+      iClear "Hregs". iRename "Hregs'" into "Hregs".
+      iDestruct (big_sepM_insert with "[$Hregs $Hr1]") as "Hregs".
+        by rewrite lookup_insert_ne // lookup_empty.
+      iDestruct (big_sepM_insert with "[$Hregs $Hr2]") as "Hregs".
+        by rewrite !lookup_insert_ne // lookup_empty.
+      iApply (wp_lea with "[$Hregs $Hi]");
+        [apply decode_encode_instrW_inv|done| |done|..].
+      { apply HPC; repeat constructor. }
+      { rewrite /regs_of /regs_of_argument !dom_insert_L dom_empty_L. set_solver-. }
+      iNext. iIntros (regs' retv) "(Hspec & ? & ?)". iDestruct "Hspec" as %Hspec.
+      destruct Hspec as [| Hfail].
+      { exfalso. simplify_map_eq. }
+      { cbn. iApply wp_pure_step_later; auto. iNext.
+        iApply wp_value. auto. } }
+    iApply (wp_lea_success_reg with "[$HPC $Hi $Hr2 $Hr1]");
+      [apply decode_encode_instrW_inv|done| |iContiguous_next Hcont 9|try done..].
+    { apply HPC; repeat constructor. }
+    iEpilogue "(HPC & Hi & Hr1 & Hr2)". iCombine "Hi" "Hprog_done" as "Hprog_done".
+    (* geta r_t1 r_t2 *)
+    destruct l as [|? l];[inversion Hprog_len|].
+    iPrologue "Hprog".
+    iApply (wp_Get_success with "[$HPC $Hi $Hr1 $Hr2]");
+      [apply decode_encode_instrW_inv|done|done| |iContiguous_next Hcont 10|auto..].
+    { apply HPC; repeat constructor. }
+    iEpilogue "(HPC & Hi & Hr2 & Hr1)". iCombine "Hi" "Hprog_done" as "Hprog_done".
+    cbn [rules_Get.denote].
+    (* move r_t4 r_t2 *)
+    destruct l as [|? l];[inversion Hprog_len|].
+    iPrologue "Hprog".
+    iApply (wp_move_success_reg with "[$HPC $Hi $Hr4 $Hr2]");
+      [apply decode_encode_instrW_inv|done| |iContiguous_next Hcont 11|auto..].
+    { apply HPC; repeat constructor. }
+    iEpilogue "(HPC & Hi & Hr4 & Hr2)". iCombine "Hi" "Hprog_done" as "Hprog_done".
+    (* subseg r_t4 r_t3 r_t1 *)
+    destruct l as [|? l];[inversion Hprog_len|].
+    iPrologue "Hprog".
+    destruct (isWithin a_m a_m' b_m e) eqn:Ha_m'_within; cycle 1.
+    { iAssert ([∗ map] k↦x ∈ (∅:gmap RegName Word), k ↦ᵣ x)%I as "Hregs'".
+        by rewrite big_sepM_empty.
+      iDestruct (big_sepM_insert with "[$Hregs' $HPC]") as "Hregs".
+        by apply lookup_empty.
+      iClear "Hregs'".
+      iDestruct (big_sepM_insert with "[$Hregs $Hr1]") as "Hregs".
+        by rewrite lookup_insert_ne // lookup_empty.
+      iDestruct (big_sepM_insert with "[$Hregs $Hr3]") as "Hregs".
+        by rewrite !lookup_insert_ne // lookup_empty.
+      iDestruct (big_sepM_insert with "[$Hregs $Hr4]") as "Hregs".
+        by rewrite !lookup_insert_ne // lookup_empty.
+      iApply (wp_Subseg with "[$Hregs $Hi]");
+        [apply decode_encode_instrW_inv|done| |done|..].
+      { apply HPC; repeat constructor. }
+      { rewrite /regs_of /regs_of_argument !dom_insert_L dom_empty_L. set_solver-. }
+      iNext. iIntros (regs' retv) "(Hspec & ? & ?)". iDestruct "Hspec" as %Hspec.
+      destruct Hspec as [| Hfail].
+      { exfalso. unfold addr_of_argument in *. simplify_map_eq.
+        repeat match goal with H:_ |- _ => apply z_to_addr_eq_inv in H end; subst.
+        congruence. }
+      { cbn. iApply wp_pure_step_later; auto. iNext. iApply wp_value. auto. } }
+    iApply (wp_subseg_success with "[$HPC $Hi $Hr4 $Hr3 $Hr1]");
+      [apply decode_encode_instrW_inv|done| |split;apply z_to_addr_z_of|try done..].
+    { apply HPC; repeat constructor. }
+    { iContiguous_next Hcont 12. }
+    iEpilogue "(HPC & Hi & Hr3 & Hr1 & Hr4)". iCombine "Hi" "Hprog_done" as "Hprog_done".
+    (* sub r_t3 r_t3 r_t1 *)
+    destruct l as [|? l];[inversion Hprog_len|].
+    iPrologue "Hprog".
+    iApply (wp_add_sub_lt_success_dst_r with "[$HPC $Hi $Hr1 $Hr3]");
+      [apply decode_encode_instrW_inv|done|iContiguous_next Hcont 13|try done..].
+    { apply HPC; repeat constructor. }
+    iEpilogue "(HPC & Hi & Hr1 & Hr3)". iCombine "Hi" "Hprog_done" as "Hprog_done".
+    cbn [denote].
+    (* lea r_t4 r_t3 *)
+    destruct l as [|? l];[inversion Hprog_len|].
+    iPrologue "Hprog".
+    iApply (wp_lea_success_reg with "[$HPC $Hi $Hr4 $Hr3]");
+      [apply decode_encode_instrW_inv|done| |iContiguous_next Hcont 14|try done..].
+    { apply HPC; repeat constructor. }
+    { transitivity (Some a_m); auto. clear; solve_addr. }
+    iEpilogue "(HPC & Hi & Hr3 & Hr4)". iCombine "Hi" "Hprog_done" as "Hprog_done".
+    (* move r_t3 r_t2 *)
+    destruct l as [|? l];[inversion Hprog_len|].
+    iPrologue "Hprog".
+    iApply (wp_move_success_reg with "[$HPC $Hi $Hr3 $Hr2]");
+      [apply decode_encode_instrW_inv|done| |iContiguous_next Hcont 15|auto..].
+    { apply HPC; repeat constructor. }
+    iEpilogue "(HPC & Hi & Hr3 & Hr2)". iCombine "Hi" "Hprog_done" as "Hprog_done".
+    (* sub r_t1 0 r_t1 *)
+    destruct l as [|? l];[inversion Hprog_len|].
+    iPrologue "Hprog".
+    iApply (wp_add_sub_lt_success_z_dst with "[$HPC $Hi $Hr1]");
+      [apply decode_encode_instrW_inv|done|iContiguous_next Hcont 16|try done..].
+    { apply HPC; repeat constructor. }
+    iEpilogue "(HPC & Hi & Hr1)". iCombine "Hi" "Hprog_done" as "Hprog_done".
+    cbn [denote].
+    (* lea r_t3 r_t1 *)
+    destruct l as [|? l];[inversion Hprog_len|].
+    iPrologue "Hprog".
+    iApply (wp_lea_success_reg with "[$HPC $Hi $Hr3 $Hr1]");
+      [apply decode_encode_instrW_inv|done| |iContiguous_next Hcont 17|try done..].
+    { apply HPC; repeat constructor. }
+    { transitivity (Some 0)%a; auto. clear; solve_addr. }
+    iEpilogue "(HPC & Hi & Hr1 & Hr3)". iCombine "Hi" "Hprog_done" as "Hprog_done".
+    (* getb r_t1 r_t3 *)
+    destruct l as [|? l];[inversion Hprog_len|].
+    iPrologue "Hprog".
+    iApply (wp_Get_success with "[$HPC $Hi $Hr1 $Hr3]");
+      [apply decode_encode_instrW_inv|done|done| |iContiguous_next Hcont 18|try done..].
+    { apply HPC; repeat constructor. }
+    iEpilogue "(HPC & Hi & Hr3 & Hr1)". iCombine "Hi" "Hprog_done" as "Hprog_done".
+    cbn [rules_Get.denote].
+    (* lea r_t3 r_t1 *)
+    destruct l as [|? l];[inversion Hprog_len|].
+    iPrologue "Hprog".
+    iApply (wp_lea_success_reg with "[$HPC $Hi $Hr3 $Hr1]");
+      [apply decode_encode_instrW_inv|done| |iContiguous_next Hcont 19|try done..].
+    { apply HPC; repeat constructor. }
+    { transitivity (Some b_m)%a; auto. clear; solve_addr. }
+    iEpilogue "(HPC & Hi & Hr1 & Hr3)". iCombine "Hi" "Hprog_done" as "Hprog_done".
+    (* store r_t3 r_t2 *)
+    destruct l as [|? l];[inversion Hprog_len|].
+    iPrologue "Hprog".
+    iApply (wp_store_success_reg with "[$HPC $Hi $Hr2 $Hr3 $Hmemptr]");
+      [apply decode_encode_instrW_inv|done|done| |iContiguous_next Hcont 20|try done..].
+    { apply HPC; repeat constructor. }
+    { split;try done. apply le_addr_withinBounds.
+      - generalize (contiguous_between_length _ _ _ Hcont). cbn.
+        clear; solve_addr.
+      - revert Hbm_am Ham_e; solve_addr. }
+    iEpilogue "(HPC & Hi & Hr2 & Hr3 & Hmemptr)". iCombine "Hi" "Hprog_done" as "Hprog_done".
+    (* move r_t1 r_t4 *)
+    destruct l as [|? l];[inversion Hprog_len|].
+    iPrologue "Hprog".
+    iApply (wp_move_success_reg with "[$HPC $Hi $Hr1 $Hr4]");
+      [apply decode_encode_instrW_inv|done| |iContiguous_next Hcont 21|auto..].
+    { apply HPC; repeat constructor. }
+    iEpilogue "(HPC & Hi & Hr1 & Hr4)". iCombine "Hi" "Hprog_done" as "Hprog_done".
+    (* move r_t2 0 *)
+    destruct l as [|? l];[inversion Hprog_len|].
+    iPrologue "Hprog".
+    iApply (wp_move_success_z with "[$HPC $Hi $Hr2]");
+      [apply decode_encode_instrW_inv|done| |iContiguous_next Hcont 22|auto..].
+    { apply HPC; repeat constructor. }
+    iEpilogue "(HPC & Hi & Hr2)". iCombine "Hi" "Hprog_done" as "Hprog_done".
+    (* move r_t3 0 *)
+    destruct l as [|? l];[inversion Hprog_len|].
+    iPrologue "Hprog".
+    iApply (wp_move_success_z with "[$HPC $Hi $Hr3]");
+      [apply decode_encode_instrW_inv|done| |iContiguous_next Hcont 23|auto..].
+    { apply HPC; repeat constructor. }
+    iEpilogue "(HPC & Hi & Hr3)". iCombine "Hi" "Hprog_done" as "Hprog_done".
+    (* move r_t4 0 *)
+    destruct l as [|? l];[inversion Hprog_len|].
+    iPrologue "Hprog".
+    iApply (wp_move_success_z with "[$HPC $Hi $Hr4]");
+      [apply decode_encode_instrW_inv|done| |iContiguous_next Hcont 24|auto..].
+    { apply HPC; repeat constructor. }
+    iEpilogue "(HPC & Hi & Hr4)". iCombine "Hi" "Hprog_done" as "Hprog_done".
+    (* jmp r_t0 *)
+    iPrologue "Hprog".
+    iApply (wp_jmp_success with "[$HPC $Hi $Hr0]");
+      [apply decode_encode_instrW_inv|done|..].
+    { apply HPC; repeat constructor. }
+    iEpilogue "(HPC & Hi & Hr0)". iCombine "Hi" "Hprog_done" as "Hprog_done".
+    (* continuation *)
+    destruct l;[|inversion Hprog_len].
+    pose proof (contiguous_between_bounds _ _ _ Hcont). 
+    assert ((a_m <= a_m')%a ∧ (a_m' <= e)%a).
+    { unfold isWithin in Ha_m'_within. (* FIXME? *)
+      rewrite andb_true_iff !Z.leb_le in Ha_m'_within |- *.
+      revert Ha_m' Hsize; clear. solve_addr. }
+    rewrite (region_addrs_zeroes_split _ a_m') //;[].
+    iDestruct (region_mapsto_split _ _ a_m' with "Hmem") as "[Hmem_fresh Hmem]"; auto.
+    { rewrite replicate_length //. }
+    iDestruct ("Hinv_close" with "[Hprog_done Hmemptr Hmem $Hna]") as ">Hna".
+    { iNext. iExists b_m, a_m'. iFrame.
+      rewrite /malloc_subroutine_instrs /malloc_subroutine_instrs'.
+      unfold region_mapsto. rewrite Hai. cbn.
+      do 25 iDestruct "Hprog_done" as "[? Hprog_done]". iFrame.
+      iPureIntro.
+      unfold isWithin in Ha_m'_within. (* FIXME? *)
+      rewrite andb_true_iff !Z.leb_le in Ha_m'_within |- *.
+      revert Ha_m' Hsize; clear; solve_addr. }
+
+    iApply (wp_wand with "[-]").
+    { iApply "Hφ". iFrame.
+      iDestruct (big_sepM_insert with "[$Hrmap $Hr4]") as "Hrmap".
+      by rewrite lookup_delete. rewrite insert_delete.
+      iDestruct (big_sepM_insert with "[$Hrmap $Hr3]") as "Hrmap".
+      by rewrite lookup_insert_ne // lookup_delete //.
+      rewrite insert_commute // insert_delete.
+      iDestruct (big_sepM_insert with "[$Hrmap $Hr2]") as "Hrmap".
+      by rewrite !lookup_insert_ne // lookup_delete //.
+      rewrite (insert_commute _ r_t2 r_t4) // (insert_commute _ r_t2 r_t3) //.
+      rewrite insert_delete.
+      rewrite (insert_commute _ r_t3 r_t2) // (insert_commute _ r_t4 r_t2) //.
+      rewrite (insert_commute _ r_t4 r_t3) //. iFrame.
+      iExists a_m, a_m', size. iFrame. repeat iSplit; auto; iPureIntro.
+      clear -H Hbm_am. solve_addr. destruct H0;auto. lia.
+    }
+    { auto. }
+  Qed.
+
+  Ltac consider_next_reg r1 r2 :=
+    destruct (decide (r1 = r2));[subst;rewrite lookup_insert;eauto|rewrite lookup_insert_ne;auto].
+
+  Lemma related_sts_pub_world_revoked_permanent W a :
+    (std W) !! a = Some Revoked →
+    related_sts_pub_world W (<s[a:=Permanent]s>W).
+  Proof.
+    intros Ha.
+    rewrite /related_sts_pub_world /=.
+    split;[|apply related_sts_pub_refl].
+    rewrite /related_sts_pub. split. 
+    - rewrite dom_insert_L. set_solver. 
+    - intros i x y Hx Hy. 
+      destruct (decide (a = i)).
+      + subst. 
+        rewrite Hx in Ha. inversion Ha.
+        rewrite lookup_insert in Hy. inversion Hy.
+        right with (Permanent);[|left]. constructor. 
+      + rewrite lookup_insert_ne in Hy;auto.
+        rewrite Hx in Hy. 
+        inversion Hy; subst.
+        left.
+  Qed.
+
+  Lemma std_update_multiple_insert_commute W a (l: list Addr) ρ ρ' :
+     a ∉ l →
+     std_update_multiple (<s[a:=ρ']s> W) l ρ = <s[a:=ρ']s> (std_update_multiple W l ρ).
+   Proof.
+     intros Hne.
+     induction l; auto; simpl.
+     apply not_elem_of_cons in Hne as [Hne Hnin]. 
+     rewrite IHl;auto. 
+     rewrite /std_update /revoke /loc /std /=. rewrite insert_commute;auto. 
+   Qed.
+  
+  Lemma related_sts_pub_update_multiple_perm W l :
+    Forall (λ k, std W !! k = Some Revoked) l →
+    related_sts_pub_world W (std_update_multiple W l Permanent).
+  Proof.
+    intros Hforall. induction l.
+    - apply related_sts_pub_refl_world. 
+    - simpl.
+      apply list.Forall_cons in Hforall as [ Ha_std Hforall].
+      eapply related_sts_pub_trans_world;[apply IHl; auto|].
+      destruct (decide (a ∈ l)).
+      { rewrite (_: <s[a:=Permanent]s>(std_update_multiple W l Permanent) = std_update_multiple W l Permanent) /=.
+          by apply related_sts_pub_refl_world.
+         rewrite /std_update insert_id /=. by destruct (std_update_multiple W l Permanent).
+           by apply std_sta_update_multiple_lookup_in_i. }
+      destruct W as [Hstd Hloc].
+      apply related_sts_pub_world_revoked_permanent in Ha_std. 
+      eapply related_sts_pub_trans_world;[apply std_update_mutiple_related_monotone,Ha_std|].
+      rewrite std_update_multiple_insert_commute //. apply related_sts_pub_refl_world. 
+  Qed.
+
+  Lemma update_region_revoked_perm E W l p v φ `{∀ Wv, Persistent (φ Wv)} :
+    (std W) !! l = Some Revoked ->
+    p ≠ O ->
+    future_priv_mono φ v -∗
+    sts_full_world W -∗
+    region W -∗
+    l ↦ₐ[p] v -∗ φ (W,v) -∗ rel l p φ ={E}=∗ region (<s[l := Permanent ]s>W)
+                             ∗ sts_full_world (<s[l := Permanent ]s>W).
+  Proof.
+    iIntros (Hrev HO) "#Hmono Hsts Hreg Hl #Hφ #Hrel".
+    rewrite region_eq /region_def.
+    iDestruct "Hreg" as (M Mρ) "(Hγrel & #Hdom & #Hdom' & Hpreds)".
+    iDestruct "Hdom" as %Hdom. iDestruct "Hdom'" as %Hdom'.
+    rewrite RELS_eq /RELS_def.
+    rewrite rel_eq /rel_def REL_eq /REL_def. iDestruct "Hrel" as (γ) "[HREL Hsaved]".
+    iDestruct (reg_in γrel (M) with "[$Hγrel $HREL]") as %HMeq.
+    rewrite /region_map_def HMeq big_sepM_insert; [|by rewrite lookup_delete].
+    iDestruct "Hpreds" as "[Hl' Hr]".
+    iDestruct "Hl'" as (ρ Hl) "[Hstate Hresources]".
+    iDestruct (sts_full_state_std with "Hsts Hstate") as %Hρ.
+    rewrite Hrev in Hρ. inversion Hρ as [Hρrev]. subst.
+    iMod (sts_update_std _ _ _ Permanent with "Hsts Hstate") as "[Hsts Hstate]".
+    assert (related_sts_pub_world W (<s[l := Permanent ]s> W)) as Hrelated.
+    { apply related_sts_pub_world_revoked_permanent; auto. }
+    iDestruct (region_map_monotone with "Hr") as "Hr";[apply Hrelated|].
+    pose proof (related_sts_pub_priv_world _ _ Hrelated) as Hrelated'.
+    iDestruct ("Hmono" $! _ _ Hrelated' with "Hφ") as "Hφ'".
+    assert (is_Some (M !! l)) as [x Hsome].
+    { apply elem_of_gmap_dom. rewrite -Hdom. apply elem_of_gmap_dom. eauto. }
+    iDestruct (region_map_delete_nonstatic with "Hr") as "Hr"; [intros m;split;intros Hcontr;congruence|].
+    iDestruct (region_map_insert_nonstatic Permanent with "Hr") as "Hr";auto.
+    iDestruct (big_sepM_delete _ _ l _ Hsome with "[Hl Hstate $Hr]") as "Hr".
+    { iExists Permanent. iFrame. iSplitR;[iPureIntro;apply lookup_insert|].
+      iExists γ, p, φ. rewrite HMeq lookup_insert in Hsome.
+      inversion Hsome. repeat (iSplit; auto). }
+    rewrite /std_update /=. iFrame "Hsts".
+    iExists M. iFrame. rewrite -HMeq. iFrame.
+    iModIntro. iExists _. iFrame. iPureIntro.
+    apply insert_id in Hsome. apply insert_id in Hl. rewrite -Hsome -Hl. split.
+    - repeat rewrite dom_insert_L;rewrite Hdom;set_solver.
+    - repeat rewrite dom_insert_L;rewrite Hdom';set_solver.
+  Qed.
+
+  Lemma extend_region_perm_sepL2_from_rev p φ E W l1 l2 `{∀ Wv, Persistent (φ Wv)}:
+     p ≠ O →
+     Forall (λ k, std W !! k = Some Revoked) l1 →
+     sts_full_world W -∗ region W -∗
+     ([∗ list] k;v ∈ l1;l2, k ↦ₐ[p] v ∗ φ (W, v) ∗ future_priv_mono φ v ∗ rel k p φ)
+
+     ={E}=∗
+
+     region (std_update_multiple W l1 Permanent)
+     ∗ ([∗ list] k ∈ l1, rel k p φ)
+     ∗ sts_full_world (std_update_multiple W l1 Permanent).
+  Proof.
+    revert l2. induction l1.
+    { cbn. intros. iIntros "? ? ?". iFrame. eauto. }
+    { intros * ? [? ?]%Forall_cons_1. iIntros "Hsts Hr Hl".
+      iDestruct (big_sepL2_length with "Hl") as %Hlen.
+      iDestruct (NoDup_of_sepL2_exclusive with "[] Hl") as %[Hal1 ND]%NoDup_cons.
+      { iIntros (? ? ?) "(H1 & ? & ?) (H2 & ? & ?)".
+        iApply (cap_duplicate_false with "[$H1 $H2]"). auto. }
+      destruct l2; [ by inversion Hlen |].
+      iDestruct (big_sepL2_cons with "Hl") as "[(Ha & Hφ & #Hf & #Hrel) Hl]".
+      iMod (IHl1 with "Hsts Hr Hl") as "(Hr & ? & Hsts)"; auto.
+      iMod (update_region_revoked_perm with "Hf Hsts Hr Ha [Hφ] Hrel") as "(? & ?)"; auto.
+      { erewrite std_sta_update_multiple_lookup_same_i;auto. }
+      { iApply ("Hf" with "[] Hφ"). iPureIntro.
+        apply related_sts_pub_priv_world,related_sts_pub_update_multiple_perm. auto. }
+      iFrame "∗ #". done. 
+    }
+  Qed.
+
+  (* dummy helper to move the later in front of the implication *)
+  Lemma helper W' g x a :
+    (∀ (r0 : leibnizO Reg) (W'0 : prodO (leibnizO (STS_std_states Addr region_type))
+                                           (leibnizO (STS_states * STS_rels))),
+        future_world g a W' W'0 → ▷ ((interp_expr interp r0) W'0) (updatePcPerm x)) -∗
+    (▷ ∀ (r0 : leibnizO Reg) (W'0 : prodO (leibnizO (STS_std_states Addr region_type))
+                                           (leibnizO (STS_states * STS_rels))),
+          future_world g a W' W'0 → ((interp_expr interp r0) W'0) (updatePcPerm x)).
+  Proof.
+    iIntros "Ha". iApply bi.later_forall. iIntros (r0). iApply bi.later_forall. iIntros (W'').
+    iSpecialize ("Ha" $! r0 W'').
+    destruct g;simpl.
+    all: iIntros (Hfuture). all: iSpecialize ("Ha" $! Hfuture);iNext;iFrame.
+  Qed.
+
+  Lemma simple_malloc_subroutine_valid W N b e :
+    Forall (λ a, W.1 !! a = Some Revoked) (region_addrs b e) →
+    na_inv logrel_nais N (malloc_inv b e) -∗
+    ([∗ list] a ∈ region_addrs b e, rel a RWX (λne Wv, interp Wv.1 Wv.2)) -∗
+    interp W (inr (E,Global,b,e,b)).
+  Proof.
+    iIntros (Hrev) "#Hmalloc #Hrels".
+    rewrite fixpoint_interp1_eq /=. iIntros (r W' Hrelated). iAlways. iNext.
+    iIntros "(#[% Hregs_valid] & Hregs & Hr & Hsts & Hown)".
+    iSplit;auto.
+    iDestruct (big_sepM_delete _ _ PC with "Hregs") as "[HPC Hregs]";[rewrite lookup_insert;eauto|].
+    destruct H with r_t0 as [? ?].
+    iDestruct (big_sepM_delete _ _ r_t0 with "Hregs") as "[r_t0 Hregs]";[rewrite !lookup_delete_ne// !lookup_insert_ne//;eauto|].
+    destruct H with r_t1 as [? ?].
+    iDestruct (big_sepM_delete _ _ r_t1 with "Hregs") as "[r_t1 Hregs]";[rewrite !lookup_delete_ne// !lookup_insert_ne//;eauto|].
+    iApply (wp_wand with "[-]").
+    iApply (simple_malloc_subroutine_spec with "[- $Hown $Hmalloc $Hregs $r_t0 $HPC $r_t1]");[|solve_ndisj|]. 
+    3: { iSimpl. iIntros (v) "[H | ->]". iExact "H". iIntros (Hcontr); done. }
+    { rewrite !dom_delete_L dom_insert_L. apply regmap_full_dom in H as <-. set_solver. }
+    iDestruct ("Hregs_valid" $! r_t0 with "[]") as "Hr0_valid";auto.
+    rewrite /RegLocate H0.
+    iDestruct (jmp_or_fail_spec with "Hr0_valid") as "Hcont".
+    destruct (decide (isCorrectPC (updatePcPerm x))).
+    2: { iNext. iIntros "(_ & _ & HPC & _)". iApply "Hcont". iFrame. iIntros (Hcontr). done. } 
+    iDestruct "Hcont" as (p g b' e' a Heq) "Hcont". simplify_eq.
+    iDestruct (helper with "Hcont") as "Hcont'".
+    iNext. iIntros "((Hown & Hregs) & Hr_t0 & HPC & Hres)".
+    iDestruct "Hres" as (ba ea size Hsizeq Hsize Hbounds Hpos) "[Hr_t1 Hbe]".
+    (* some usefull lemmas about [ba ea] *)
+    assert (∃ l1 l2, region_addrs b e = l1 ++ region_addrs ba ea ++ l2) as [l1 [l2 Heqapp] ].
+    { exists (region_addrs b ba),(region_addrs ea e).
+      rewrite -region_addrs_split;[|solve_addr].
+      rewrite -region_addrs_split;[auto|solve_addr]. }
+    (* The following lemma can be derived from the fact that we own the resources for ba,ea, which means they cannot
+       be in region W' *)
+    iAssert (⌜Forall (λ k : Addr, std W' !! k = Some Revoked) (region_addrs ba ea)⌝)%I as %Hrev'.
+    { rewrite Heqapp in Hrev. apply Forall_app in Hrev as [_ Hrev]. apply Forall_app in Hrev as [Hrev _].
+      revert Hrev. rewrite !Forall_forall. iIntros (Hrev x Hin). specialize (Hrev x Hin).
+      pose proof (related_sts_priv_world_std_sta_is_Some W W' x Hrelated) as [ρ Hρ];[eauto|].
+      rewrite /region_mapsto.
+      iDestruct (big_sepL_elem_of _ _ x with "Hrels") as "Hrel".
+      { rewrite Heqapp. apply elem_of_app. right. apply elem_of_app. by left. }
+      apply elem_of_list_lookup in Hin as [k Hk].
+      iDestruct (big_sepL2_extract_l with "Hbe") as "[_ Hb]";[eauto|].
+      iDestruct "Hb" as (w') "Hw'".
+      destruct ρ;auto. (* all the following will lead to duplicate resources for x *)
+      - iDestruct (region_open_temp_nwl with "[$Hrel $Hr $Hsts]") as (v) "(_ & _ & _ & Hw & _)";[eauto|auto|..].
+        iDestruct (cap_duplicate_false with "[$Hw' $Hw]") as "?";auto.
+      - iDestruct (region_open_monotemp_nwl with "[$Hrel $Hr $Hsts]") as (v) "(_ & _ & _ & Hw & _)";[eauto|auto|..].
+        iDestruct (cap_duplicate_false with "[$Hw' $Hw]") as "?";auto.
+      - iDestruct (region_open_perm with "[$Hrel $Hr $Hsts]") as (v) "(_ & _ & _ & Hw & _)";[eauto|auto|..].
+        iDestruct (cap_duplicate_false with "[$Hw' $Hw]") as "?";auto.
+      - iMod (region_invariants_static.region_open_static with "[$Hr $Hsts]") as "(_ & _ & ? & H & %)";[apply Hρ|..].
+        rewrite /region_invariants_static.static_resources.
+        apply elem_of_gmap_dom in H2 as [? Hx].
+        iDestruct (big_sepM_delete with "H") as "[H ?]";[apply Hx|].
+        iDestruct "H" as (? ?) "[HH Hw]". iDestruct (rel_agree _ H2 with "[$Hrel $HH]") as "(% & _)";subst. 
+        iDestruct (cap_duplicate_false with "[$Hw' $Hw]") as "?";auto.
+      - iMod (region_invariants_static.region_open_monostatic with "[$Hr $Hsts]") as "(_ & _ & ? & H & %)";[apply Hρ|..].
+        rewrite /region_invariants_static.static_resources.
+        apply elem_of_gmap_dom in H2 as [? Hx].
+        iDestruct (big_sepM_delete with "H") as "[H ?]";[apply Hx|].
+        iDestruct "H" as (? ?) "[HH Hw]". iDestruct (rel_agree _ H2 with "[$Hrel $HH]") as "(% & _)";subst. 
+        iDestruct (cap_duplicate_false with "[$Hw' $Hw]") as "?";auto.
+      - iDestruct (region_open_uninitialized with "[$Hrel $Hr $Hsts]") as "(_ & _ & _ & Hw & _)";[eauto|auto|..].
+        iDestruct (cap_duplicate_false with "[$Hw' $Hw]") as "?";auto.
+    }
+    (* Next is the interesting part of the spec: we must allocate the invariants making the malloced region valid *)
+    iMod (extend_region_perm_sepL2_from_rev RWX (λ Wv, interp Wv.1 Wv.2) _ _
+                                            (region_addrs ba ea)
+                                            (region_addrs_zeroes ba ea) with "Hsts Hr [Hbe]") as "(Hr & #Hvalid & Hsts)";auto.
+    { rewrite Heqapp.
+      iDestruct (big_sepL_app with "Hrels") as "[_ Hrels']". 
+      iDestruct (big_sepL_app with "Hrels'") as "[Hrels'' _]". 
+      iDestruct (big_sepL2_to_big_sepL_l _ _ (region_addrs_zeroes ba ea) with "Hrels''") as "Hrels3".
+      { by rewrite /region_addrs_zeroes region_addrs_length replicate_length. }
+      iDestruct (big_sepL2_sep with "[Hrels3 Hbe]") as "Hbe";[iFrame "Hbe"; iFrame "Hrels3"|].
+      iApply (big_sepL2_mono with "Hbe").
+      iIntros (k a' w Hin1 Hin2) "(Ha & Hrel)". iFrame.
+      apply region_addrs_zeroes_lookup in Hin2 as ->. iSplit.
+      - by rewrite fixpoint_interp1_eq /=.
+      - iAlways. iIntros (W1 W2 Hrelated') "Hv /=". by rewrite !fixpoint_interp1_eq /=.
+    }
+    rewrite -!(delete_insert_ne _ r_t1)//.
+    iDestruct (big_sepM_insert with "[$Hregs $Hr_t1]") as "Hregs";[apply lookup_delete|rewrite insert_delete].
+    rewrite -!(delete_insert_ne _ r_t0)//.
+    iDestruct (big_sepM_insert with "[$Hregs $Hr_t0]") as "Hregs";[apply lookup_delete|rewrite insert_delete delete_insert_delete].
+    rewrite -!(delete_insert_ne _ PC)//.
+    iDestruct (big_sepM_insert with "[$Hregs $HPC]") as "Hregs";[apply lookup_delete|rewrite insert_delete].
+    set regs := <[PC:=updatePcPerm (inr (p, g, b', e', a))]>
+                            (<[r_t0:=inr (p, g, b', e', a)]> (<[r_t1:=inr (RWX, Global, ba, ea, ba)]> (<[r_t2:=inl 0%Z]> (<[r_t3:=inl 0%Z]> (<[r_t4:=inl 0%Z]> r))))).
+    iDestruct ("Hcont'" $! regs with "[] [$Hown Hregs $Hr $Hsts]") as "[_ Hcont'']".
+    { destruct g; iPureIntro;[apply related_sts_pub_priv_world|
+                              apply related_sts_pub_pub_plus_world|
+                              apply related_sts_pub_a_world]; try apply related_sts_pub_update_multiple_perm;auto. }
+    { rewrite /regs. iSplitR "Hregs".
+      - iSplit.
+        + iPureIntro. intros x. consider_next_reg x PC. consider_next_reg x r_t0. consider_next_reg x r_t1.
+          consider_next_reg x r_t2. consider_next_reg x r_t3. consider_next_reg x r_t4.
+        + iIntros (x Hne). rewrite /RegLocate. consider_next_reg x PC;[contradiction|].
+          consider_next_reg x r_t0.
+          { iDestruct ("Hregs_valid" $! r_t0 with "[]") as "Hr0_valid'";auto. rewrite H0.
+            iApply (interp_monotone with "[] Hr0_valid'"). iPureIntro. apply related_sts_pub_update_multiple_perm;auto. }
+          consider_next_reg x r_t1.
+          { rewrite !fixpoint_interp1_eq. iApply (big_sepL_mono with "Hvalid").
+            iIntros (k y Hky) "Ha". iExists RWX. iFrame. iSplit;auto. iPureIntro. simpl.
+            rewrite std_sta_update_multiple_lookup_in_i;auto.
+            apply elem_of_list_lookup. exists k. auto. 
+          }
+          consider_next_reg x r_t2. by rewrite !fixpoint_interp1_eq.
+          consider_next_reg x r_t3. by rewrite !fixpoint_interp1_eq.
+          consider_next_reg x r_t4. by rewrite !fixpoint_interp1_eq.
+          iSpecialize ("Hregs_valid" $! _ Hne).
+          iApply (interp_monotone with "[] Hregs_valid"). iPureIntro. apply related_sts_pub_update_multiple_perm;auto.
+      - rewrite insert_insert. iFrame. 
+    }
+    iApply (wp_wand with "Hcont''").
+    iIntros (v) "HH". iIntros (Hv).
+    iDestruct ("HH" $! Hv) as (? ?) "(Hfull & Hvals & % & Hown & Hsts & Hr)".
+    iExists _,_. iFrame. iPureIntro.
+    eapply related_sts_priv_trans_world;[|apply H4].
+    apply related_sts_pub_priv_world. apply related_sts_pub_update_multiple_perm;auto.
+  Qed.
+
+
+End SimpleMalloc.
+
