theories/examples/macros/rclear.v
@@ -1,0 +1,187 @@
+From iris.algebra Require Import frac.
+From iris.proofmode Require Import tactics.
+Require Import Eqdep_dec List.
+From cap_machine Require Import rules.
+From cap_machine Require Export iris_extra addr_reg_sample region_macros contiguous stack_macros_helpers.
+
+Section stack_macros.
+  Context {Σ:gFunctors} {memg:memG Σ} {regg:regG Σ}
+          `{MonRef: MonRefG (leibnizO _) CapR_rtc Σ}
+          `{MP: MachineParameters}.
+
+  (* -------------------------------------- RCLEAR ----------------------------------- *)
+  (* the following macro clears registers in r. a denotes the list of addresses
+     containing the instructions for the clear: |a| = |r| *)
+     Definition rclear_instrs (r : list RegName) := map (λ r_i, move_z r_i 0) r.
+
+     Lemma rclear_instrs_cons rr r: rclear_instrs (rr :: r) = move_z rr 0 :: rclear_instrs r.
+     Proof. reflexivity. Qed.
+
+     Definition rclear (a : list Addr) (p : Perm) (r : list RegName) : iProp Σ :=
+         ([∗ list] k↦a_i;w_i ∈ a;(rclear_instrs r), a_i ↦ₐ[p] w_i)%I.
+
+     Lemma rclear_spec (a : list Addr) (r: list RegName) (rmap : gmap RegName Word) p p' g b e a1 an φ :
+       contiguous_between a a1 an →
+       ¬ PC ∈ r → hd_error a = Some a1 →
+       isCorrectPC_range p g b e a1 an →
+       PermFlows p p' →
+       list_to_set r = dom (gset RegName) rmap →
+
+         ▷ ([∗ map] r_i↦w_i ∈ rmap, r_i ↦ᵣ w_i)
+       ∗ ▷ PC ↦ᵣ inr ((p,g),b,e,a1)
+       ∗ ▷ rclear a p' r
+       ∗ ▷ (PC ↦ᵣ inr ((p,g),b,e,an) ∗ ([∗ map] r_i↦_ ∈ rmap, r_i ↦ᵣ inl 0%Z)
+               ∗ rclear a p' r -∗
+               WP Seq (Instr Executable) {{ φ }})
+       ⊢ WP Seq (Instr Executable) {{ φ }}.
+     Proof.
+       iIntros (Ha Hne Hhd Hvpc Hfl Hrdom) "(>Hreg & >HPC & >Hrclear & Hφ)".
+       iDestruct (big_sepL2_length with "Hrclear") as %Har.
+       iRevert (Hne Har Hhd Hvpc Ha Hrdom).
+       iInduction (a) as [| a1'] "IH" forall (r rmap a1 an).
+       { iIntros (Hne Har Hhd Hvpc Ha Hrdom). by inversion Hhd; simplify_eq. }
+       iIntros (Hne Har Hhd Hvpc Ha Hrdom).
+       iApply (wp_bind (fill [SeqCtx])). rewrite /rclear /=.
+       (* rewrite -(beq_nat_refl (length r)).  *)destruct r; inversion Har.
+       rewrite rclear_instrs_cons.
+       iDestruct (big_sepL2_cons with "Hrclear") as "[Ha1 Hrclear]".
+       rewrite list_to_set_cons in Hrdom.
+       assert (is_Some (rmap !! r)) as [rv ?].
+       { rewrite elem_of_gmap_dom -Hrdom. set_solver. }
+       iDestruct (big_sepM_delete _ _ r with "Hreg") as "[Hr Hreg]". eauto.
+       pose proof (contiguous_between_cons_inv _ _ _ _ Ha) as [-> [a2 [? Hcont'] ] ].
+       iApply (wp_move_success_z with "[$HPC $Hr $Ha1]");
+         [apply decode_encode_instrW_inv|apply Hfl|iCorrectPC a1 an|eauto|..].
+       iNext. iIntros "(HPC & Ha1 & Hr)". iApply wp_pure_step_later; auto. iNext.
+       destruct a.
+       { iApply "Hφ". iFrame. inversion Hcont'; subst. iFrame.
+         destruct r0; inversion Har. simpl in Hrdom.
+         iApply (big_sepM_delete _ _ r). eauto.
+         rewrite (_: delete r rmap = ∅). rewrite !big_sepM_empty. eauto.
+         apply map_empty. intro. eapply (@not_elem_of_dom _ _ (gset RegName)).
+         typeclasses eauto. rewrite dom_delete_L -Hrdom. set_solver. }
+
+       pose proof (contiguous_between_cons_inv_first _ _ _ _ Hcont') as ->.
+       assert (PC ∉ r0). { apply not_elem_of_cons in Hne as [? ?]. auto. }
+
+       destruct (decide (r ∈ r0)).
+       { iDestruct (big_sepM_insert with "[$Hreg $Hr]") as "Hreg".
+           by rewrite lookup_delete. rewrite insert_delete.
+         iApply ("IH" with "Hreg HPC Hrclear [Hφ Ha1]"); eauto.
+         { iNext. iIntros "(? & Hreg & ?)". iApply "Hφ". iFrame.
+           iApply (big_sepM_delete _ _ r). eauto.
+           iDestruct (big_sepM_delete _ _ r with "Hreg") as "[? ?]".
+           rewrite lookup_insert //. iFrame. rewrite delete_insert_delete //. }
+         { iPureIntro. intros ? [? ?]. apply Hvpc. solve_addr. }
+         { iPureIntro. rewrite dom_insert_L -Hrdom. set_solver. } }
+       { iApply ("IH" with "Hreg HPC Hrclear [Hφ Ha1 Hr]"); eauto.
+         { iNext. iIntros "(? & ? & ?)". iApply "Hφ". iFrame.
+           iApply (big_sepM_delete _ _ r). eauto. iFrame. }
+         { iPureIntro. intros ? [? ?]. apply Hvpc. solve_addr. }
+         { iPureIntro. rewrite dom_delete_L -Hrdom. set_solver. } }
+     Qed.
+
+     (* Lemma used to fit the rclear spec to the value relation *)
+     Lemma rmap_zero_extract (rmap : Reg) :
+       ([∗ map] r_i↦_ ∈ rmap, r_i ↦ᵣ inl 0%Z) -∗
+       ∃ rmap', ([∗ map] r_i↦y ∈ rmap', r_i ↦ᵣ y %Z) ∗ ⌜dom (gset RegName) rmap' = dom (gset RegName) rmap ∧ (∀ x : RegName, x ∈ (dom (gset RegName) rmap') → rmap' !! x = Some (inl 0)%Z)⌝.
+     Proof.
+       iIntros "Hmap".
+       assert (∃ rlist, map_to_list rmap ≡ₚ rlist) as [rlist HPerm]. eexists; eauto.
+       pose proof (NoDup_fst_map_to_list rmap) as HnoDup.
+       iRevert (HPerm HnoDup). iInduction (rlist) as [| a_head a_tail] "IH" forall (rmap); iIntros (HPerm HnoDup).
+       - iExists ∅. apply (map_to_list_empty_inv_alt rmap) in HPerm as ->. auto.
+       - eapply NoDup_map_to_cons in HnoDup; eauto.
+         destruct a_head.
+         apply (map_to_list_insert_inv rmap) in HPerm as ->.
+         cbn in HnoDup. inversion HnoDup as [| r' l' Hne HdoDup]. simplify_eq.
+         iDestruct (big_sepM_insert with "Hmap") as "[Ha Htail]".
+         {
+           apply not_elem_of_list_to_map_1.
+           revert Hne; clear. induction a_tail.
+           - intros H HFalse. by inversion HFalse.
+           - intros HnotIn. rewrite fmap_cons.
+             rewrite !not_elem_of_cons in HnotIn |- * => HnotIn. destruct HnotIn as [Hnota HnotTail].
+             split; auto. }
+
+         iSpecialize ("IH" $! (list_to_map a_tail) with "Htail").
+         assert (map_to_list (list_to_map a_tail) ≡ₚ a_tail) as Hinv.
+         { apply map_to_list_to_map. done. }
+         unshelve iSpecialize ("IH" $! Hinv _).
+         { rewrite map_to_list_to_map; auto. }
+         iDestruct "IH" as  (rmap0) "[Heq' [HnoDup' IH]]".
+         iExists (<[r:=inl 0%Z]> rmap0).
+         iSplitL "Ha Heq'".
+         iAssert (⌜rmap0 !! r = None⌝)%I as %HrNone.
+         { destruct (rmap0!!r) eqn:Hr; last auto.
+           iDestruct (big_sepM_delete with "Heq'") as "[Heq' _]"; eauto.
+           iDestruct (regname_dupl_false with "Ha Heq'") as "HFalse"; auto.
+         }
+         iDestruct (big_sepM_insert with "[$Heq' $Ha]") as "Hmap"; eauto.
+         iSplitL "HnoDup'".
+         + rewrite !dom_insert_L. iDestruct "HnoDup'" as %->. iPureIntro. reflexivity.
+         + iDestruct "IH" as %IH. iPureIntro. intros x Hdom.
+           destruct (decide (r = x)).
+           ++ simplify_eq; by rewrite /RegLocate lookup_insert.
+           ++ rewrite /RegLocate lookup_insert_ne; [|auto].
+               rewrite dom_insert_L elem_of_union in Hdom |- * => Hdom.
+               destruct Hdom as [Hsin | Hrest].
+           * apply elem_of_singleton in Hsin. simpl in Hsin. simplify_map_eq.
+             apply elem_of_singleton in Hsin. congruence.
+           * specialize (IH x Hrest); auto.
+       Qed.
+
+   (* Slightly shorter, constructive version of the same proof, that requires an auxiliary list. *)
+     Lemma rmap_zero_extract_list (rmap : Reg) l :
+       dom (gset RegName) rmap = (list_to_set l : gset RegName) → ([∗ map] r_i↦_ ∈ rmap, r_i ↦ᵣ inl 0%Z) -∗
+       ∃ rmap', ([∗ map] r_i↦y ∈ rmap', r_i ↦ᵣ y %Z) ∗ ⌜dom (gset RegName) rmap' = list_to_set l ∧ (∀ x : RegName, x ∈ (dom (gset RegName) rmap') → rmap' !! x = Some (inl 0)%Z)⌝.
+     Proof.
+       set (rmap' := ((create_gmap_default l (inl 0%Z : Word)) : Reg)).
+       iIntros (Hdom) "Hmap".
+       iExists rmap'.
+       iSplitL.
+       - iApply (big_sepM_mono (λ k _, k ↦ᵣ inl 0%Z))%I.
+         {
+           iIntros (k x Hcreate) "Hzero".
+           pose proof (create_gmap_default_dom l (inl 0%Z : Word)) as Hdom'.
+           assert (k ∈ l) as HkDom.
+           { assert (k ∈ (list_to_set l : gset RegName) ). rewrite -Hdom'. eapply elem_of_dom_2; eauto. apply (elem_of_list_to_set k l) in H; auto. }
+           rewrite (create_gmap_default_lookup _ (inl 0%Z : Word) k) in HkDom |- * => HkDom. subst rmap'.
+           rewrite Hcreate in HkDom. inversion HkDom; done.
+         }
+         rewrite !big_sepM_dom.
+         rewrite create_gmap_default_dom Hdom. iExact "Hmap".
+       - iPureIntro. split.
+         * by rewrite create_gmap_default_dom.
+         * intros x Hxdom. subst rmap'.
+           rewrite create_gmap_default_dom (elem_of_list_to_set _ l) in Hxdom |- * => HxDom.
+           rewrite /RegLocate. apply (create_gmap_default_lookup l (inl 0%Z :Word) x) in HxDom. by rewrite HxDom.
+     Qed.
+
+     (* rclear spec in terms of a new map; this one should be a bit more practical in proofs - should also help rewrite parts of the awkward example *)
+     Lemma rclear_spec_gmap (a : list Addr) (r: list RegName) (rmap : gmap RegName Word) p p' g b e a1 an φ :
+     contiguous_between a a1 an →
+     ¬ PC ∈ r → hd_error a = Some a1 →
+     isCorrectPC_range p g b e a1 an →
+     PermFlows p p' →
+     list_to_set r = dom (gset RegName) rmap →
+   
+       ▷ ([∗ map] r_i↦w_i ∈ rmap, r_i ↦ᵣ w_i)
+     ∗ ▷ PC ↦ᵣ inr ((p,g),b,e,a1)
+     ∗ ▷ rclear a p' r
+     ∗ ▷ (PC ↦ᵣ inr ((p,g),b,e,an) ∗
+             (∃ rmap', ([∗ map] r_i↦y ∈ rmap', r_i ↦ᵣ y %Z) ∗ ⌜dom (gset RegName) rmap' = (list_to_set r) ∧ (∀ x : RegName, x ∈ (dom (gset RegName) rmap') → rmap' !! x = Some (inl 0%Z))⌝)
+             ∗ rclear a p' r -∗
+             WP Seq (Instr Executable) {{ φ }})
+     ⊢ WP Seq (Instr Executable) {{ φ }}.
+   Proof.
+     iIntros (Ha Hne Hhd Hvpc Hfl Hrdom) "(>Hreg & >HPC & >Hrclear & Hφ)".
+     iApply (rclear_spec with "[- $Hreg $HPC $Hrclear]"); eauto.
+     iNext. iIntros "(HPC & Hreg & Hrclear)".
+     iDestruct (rmap_zero_extract with "Hreg") as "Hreg'"; auto.
+     iDestruct "Hreg'" as (rmap') "(Hreg & Hdom & Hinl0)".
+     rewrite -Hrdom.
+     iApply "Hφ". iFrame. iExists rmap'. iFrame. iSplitL "Hdom"; iFrame.
+   Qed.
+
+End stack_macros.
