theories/examples/stack_macros_helpers.v
@@ -50,4 +50,202 @@ Section helpers.
       congruence.
   Qed.
 
+  Lemma isCorrectPC_range_restrict p g b e a0 an a0' an' :
+    isCorrectPC_range p g b e a0 an →
+    (a0 <= a0')%a ∧ (an' <= an)%a →
+    isCorrectPC_range p g b e a0' an'.
+  Proof.
+    intros HR [? ?] a' [? ?]. apply HR. solve_addr.
+  Qed.
+
+  Lemma isCorrectPC_range_monotone p g b e a0 an a' a'':
+    isCorrectPC_range p g b e a0 an →
+    (a0 <= a')%a → (a'' <= an)%a →
+    isCorrectPC_range p g b e a' a''.
+  Proof.
+    intros. intros a1 [Ha'1 Ha'2]. apply H. solve_addr.
+  Qed.
+
+  Lemma isCorrectPC_range_split :
+    ∀ (p : Perm) (g : Locality) (b e a0 an a_link : Addr),
+      isCorrectPC_range p g b e a0 an
+      → (a0 <= a_link)%a → (a_link <= an)%a →
+      isCorrectPC_range p g b e a0 a_link ∧ isCorrectPC_range p g b e a_link an.
+  Proof.
+    intros * HCorr ??. split; eapply isCorrectPC_range_monotone; eauto; solve_addr.
+  Qed.
+  
+  Lemma pc_range_not_E  pc_p pc_g pc_b pc_e a_first a_last a_tail:
+    isCorrectPC_range pc_p pc_g pc_b pc_e a_first a_last →
+    contiguous_between (a_first :: a_tail) a_first a_last →
+    pc_p ≠ E.
+  Proof.
+    intros Hvpc Hcont.
+    apply isCorrectPC_range_perm in Hvpc as [Heq | [Heq | Heq] ]; subst; auto.
+    apply (contiguous_between_middle_bounds _ 0 a_first) in Hcont as [_ Hlt]; auto.
+  Qed.
+
+  Lemma pc_range_perm  pc_p pc_g pc_b pc_e a_first a_last a_tail:
+    isCorrectPC_range pc_p pc_g pc_b pc_e a_first a_last →
+    contiguous_between (a_first :: a_tail) a_first a_last →
+    pc_p = RX ∨ pc_p = RWX ∨ pc_p = RWLX.
+  Proof.
+    intros Hvpc Hcont.
+    apply isCorrectPC_range_perm in Hvpc as [Heq | [Heq | Heq] ]; subst; auto.
+    apply (contiguous_between_middle_bounds _ 0 a_first) in Hcont as [_ Hlt]; auto.
+  Qed.
+
+  Lemma pc_range_nonO  pc_p pc_g pc_b pc_e a_first a_last a_tail:
+    isCorrectPC_range pc_p pc_g pc_b pc_e a_first a_last →
+    contiguous_between (a_first :: a_tail) a_first a_last →
+    pc_p ≠ O.
+  Proof.
+    intros Hcorr Hcont.
+    assert (pc_p = RX ∨ pc_p = RWX ∨ pc_p = RWLX) as [-> | [-> | ->] ] by (eapply pc_range_perm; eauto); auto.
+  Qed.
+
+  Lemma pc_range_readA  pc_p pc_g pc_b pc_e a_first a_last a_tail:
+    isCorrectPC_range pc_p pc_g pc_b pc_e a_first a_last →
+    contiguous_between (a_first :: a_tail) a_first a_last →
+    readAllowed pc_p = true.
+  Proof.
+    intros Hcorr Hcont.
+    assert (pc_p = RX ∨ pc_p = RWX ∨ pc_p = RWLX) as [-> | [-> | ->] ] by (eapply pc_range_perm; eauto); auto.
+  Qed.
+
 End helpers.
+
+(* -------------------------------- LTACS ------------------------------------------- *)
+
+  (* Destructing -parts of- sequences of addresses *)
+  Ltac prep_addr_core list n :=
+    match eval compute in n with
+    | 0 => idtac
+    | _ => destruct list;[done|]; prep_addr_core list (pred n) end.
+
+  Ltac prep_addr_list list Hcont n :=
+    let l := fresh "l" in
+    destruct list as [| list l];[done|];
+    apply contiguous_between_cons_inv_first in Hcont as Heq; subst list;
+    prep_addr_core l (pred n).
+
+  Ltac destruct_addr_list list :=
+    let l := fresh "l" in
+    destruct list as [| list l];[done|];
+    repeat (destruct l;[done|]); destruct l; [|done].
+
+  Ltac prep_addr_list_full list Hcont :=
+    destruct_addr_list list;
+    apply contiguous_between_cons_inv_first in Hcont as Heq; subst list.
+
+  (* Tactics for single instruction spec application *)
+  Ltac iPrologue_pre :=
+    match goal with
+    | Hlen : length ?a = ?n |- _ =>
+      let a' := fresh "a" in
+      destruct a as [| a' a]; inversion Hlen; simpl
+    end.
+
+  Ltac iPrologue prog :=
+    let str_destr := constr:(("[Hi " ++ prog ++ "]")%string) in
+    iDestruct prog as str_destr;
+    iApply (wp_bind (fill [SeqCtx])).
+
+  Ltac iEpilogue prog :=
+    iNext; iIntros prog; iSimpl;
+    iApply wp_pure_step_later;auto;iNext.
+
+  Ltac iEpilogueLoad z prog :=
+    iNext; iIntros (z) prog; iSimpl;
+    iApply wp_pure_step_later;auto;iNext.
+
+  Ltac iCorrectPC i j :=
+    eapply isCorrectPC_contiguous_range with (a0 := i) (an := j); eauto; [];
+    cbn; solve [ repeat constructor ].
+
+  Ltac iContiguous_next Ha index :=
+    apply contiguous_of_contiguous_between in Ha;
+    generalize (contiguous_spec _ Ha index); auto.
+
+  Lemma lst_lkup_head `{A : Type} hd (tail : list A) :
+    (hd :: tail) !! 0 = Some hd.
+  Proof. done. Qed.
+  Lemma lst_lkup_cons `{A : Type} hd (tail : list A) i:
+    (hd :: tail) !! (i + 1) = tail !! i.
+  Proof. rewrite -plus_n_Sm Nat.add_0_r. rewrite -lookup_tail. simpl. done. Qed.
+  Ltac iContiguous_next_a Ha :=
+    apply contiguous_of_contiguous_between in Ha;
+    eapply (contiguous_spec _ Ha);
+    [repeat first [ by apply lst_lkup_head | erewrite lst_lkup_cons ] | done].
+  Ltac iCorrectPC_a :=
+    match goal with
+    | _ : isCorrectPC_range _ _ _ _ ?i ?j |- _ =>
+      eapply isCorrectPC_contiguous_range with (a0 := i) (an := j); eauto; [];
+      cbn; solve [ repeat constructor ]
+    end.
+
+  Ltac contiguous_between_clean Hcont :=
+    repeat apply contiguous_between_weak in Hcont.
+
+  (* Tactics in case of CPS spec *)
+  Ltac derive_length Hprog Hprog_len :=
+    iDestruct (big_sepL2_length with Hprog) as %Hprog_len; simpl in Hprog_len.
+  Ltac split_program Hprog Hcont a_link :=
+    let str_destr := constr:(("(Hcode & " ++ Hprog ++ " & #Hcontig)")%string) in
+    let l_code := fresh "l_code" in
+    let l_rest := fresh "l_rest" in
+    iDestruct (contiguous_between_program_split with Hprog) as (l_code l_rest a_link)  str_destr;[apply Hcont|]; clear Hcont.
+  Ltac split_PC_range Hvpc Hcont_code Hcont a_linka :=
+    let Hvpc_code := fresh "Hvpc_code" in
+    let Hvpc_rest := fresh "Hvpc_rest" in
+    edestruct isCorrectPC_range_split with (a_link := a_linka) as [Hvpc_code Hvpc_rest];[exact Hvpc| apply (contiguous_between_bounds _ _ _ Hcont_code) | apply (contiguous_between_bounds _ _ _ Hcont)| ..]; clear Hvpc; rename Hvpc_rest into Hvpc.
+
+  Ltac iPrologue_multi Hprog Hcont Hvpc a_link :=
+    split_program Hprog Hcont a_link;
+    let Hcont_code := fresh "Hcont_code" in
+    let Hlink := fresh "Hlink" in
+    let Hre := fresh "Hre" in
+    iDestruct "Hcontig" as %(Hcont_code & Hcont & Hre & Hlink);
+    rewrite -> Hre in *; clear Hre;
+    let Hlength_code := fresh "Hlength_code" in
+    derive_length "Hcode" Hlength_code;
+    rewrite Hlength_code in Hlink; clear Hlength_code;
+    let Hlength := fresh "Hlength" in
+    derive_length Hprog Hlength;
+    split_PC_range Hvpc Hcont_code Hcont a_link.
+
+  Tactic Notation "iEpilogue_multi" constr(Hprog) hyp_list(Hclear) :=
+    let Hfresh := fresh "Hfresh" in
+    assert (Hfresh : True) by auto;
+    iNext; iIntros Hprog; clear Hfresh Hclear.
+
+  Ltac frame_conjunction Hyp :=
+    repeat (iDestruct Hyp as "[Hi Hprog_done]"; iFrame "Hi"); iFrame; auto.
+
+  (* Adding and removing pointso from a map *)
+
+ Ltac extract_pointsto_map regs Hmap rname Hrdom Hreg :=
+    let rval := fresh "v"rname in
+    let Hsome := fresh "Hsome" in
+    let str_destr := constr:(("[" ++ Hreg ++ " " ++ Hmap ++ "]")%string) in
+    assert (is_Some (regs !! rname)) as [rval Hsome] by (apply Hrdom; repeat constructor);
+    iDestruct (big_sepM_delete _ _ rname with Hmap) as str_destr; first by simplify_map_eq.
+  Ltac solve_insert_dom :=
+  rewrite -(not_elem_of_dom (D := (gset RegName)));
+  match goal with
+  | [ H : dom (gset RegName) _ = _ |- _ ] =>
+    rewrite H end;
+  set_solver+.
+
+  Ltac insert_pointsto_map_dom Hmap Hreg:=
+    let str_destr := constr:(("[ $" ++ Hmap ++ " $" ++ Hreg ++ "]")%string) in
+    iDestruct (big_sepM_insert with str_destr) as Hmap;
+    [(repeat rewrite lookup_insert_ne //;[]); solve_insert_dom | ].
+
+  Ltac insert_pointsto_map_del Hmap Hreg :=
+    let str_destr := constr:(("[ $" ++ Hmap ++ " $" ++ Hreg ++ "]")%string) in
+    iDestruct (big_sepM_insert with str_destr) as Hmap;
+    [by simplify_map_eq | repeat (rewrite -delete_insert_ne //;[]); try rewrite insert_delete].
+
+   Ltac insert_pointsto_map Hmap Hreg :=
+     first [insert_pointsto_map_del Hmap Hreg | insert_pointsto_map_dom Hmap Hreg].
