theories/rules/rules_Mov.v
@@ -95,7 +95,6 @@ Section cap_lang_rules.
     PermFlows pc_p pc_p' →
     isCorrectPC (inr ((pc_p,pc_g),pc_b,pc_e,pc_a)) →
     (pc_a + 1)%a = Some pc_a' →
-    PC ≠ r1 →
 
     {{{ ▷ PC ↦ᵣ inr ((pc_p,pc_g),pc_b,pc_e,pc_a)
         ∗ ▷ pc_a ↦ₐ[pc_p'] w
@@ -106,7 +105,7 @@ Section cap_lang_rules.
           ∗ pc_a ↦ₐ[pc_p'] w
           ∗ r1 ↦ᵣ inl z }}}.
   Proof.
-    iIntros (Hinstr Hfl Hvpc Hpca' Hne ϕ) "(>HPC & >Hpc_a & >Hr1) Hφ".
+    iIntros (Hinstr Hfl Hvpc Hpca' ϕ) "(>HPC & >Hpc_a & >Hr1) Hφ".
     iDestruct (map_of_regs_2 with "HPC Hr1") as "[Hmap %]".
     iApply (wp_Mov with "[$Hmap Hpc_a]"); eauto; simplify_map_eq; eauto.
     by unfold regs_of; rewrite !dom_insert; set_solver+.
@@ -126,7 +125,6 @@ Section cap_lang_rules.
     PermFlows pc_p pc_p' →
     isCorrectPC (inr ((pc_p,pc_g),pc_b,pc_e,pc_a)) →
     (pc_a + 1)%a = Some pc_a' →
-    PC ≠ r1 →
 
     {{{ ▷ PC ↦ᵣ inr ((pc_p,pc_g),pc_b,pc_e,pc_a)
         ∗ ▷ pc_a ↦ₐ[pc_p'] w
@@ -139,7 +137,7 @@ Section cap_lang_rules.
           ∗ r1 ↦ᵣ wrv
           ∗ rv ↦ᵣ wrv }}}.
   Proof.
-    iIntros (Hinstr Hfl Hvpc Hpca' Hne ϕ) "(>HPC & >Hpc_a & >Hr1 & >Hrv) Hφ".
+    iIntros (Hinstr Hfl Hvpc Hpca' ϕ) "(>HPC & >Hpc_a & >Hr1 & >Hrv) Hφ".
     iDestruct (map_of_regs_3 with "HPC Hr1 Hrv") as "[Hmap (%&%&%)]".
     iApply (wp_Mov with "[$Hmap Hpc_a]"); eauto; simplify_map_eq; eauto.
     by unfold regs_of; rewrite !dom_insert; set_solver+.
@@ -159,7 +157,6 @@ Section cap_lang_rules.
     PermFlows pc_p pc_p' →
     isCorrectPC (inr ((pc_p,pc_g),pc_b,pc_e,pc_a)) →
     (pc_a + 1)%a = Some pc_a' →
-    PC ≠ r1 →
 
     {{{ ▷ PC ↦ᵣ inr ((pc_p,pc_g),pc_b,pc_e,pc_a)
         ∗ ▷ pc_a ↦ₐ[pc_p'] w
@@ -170,7 +167,7 @@ Section cap_lang_rules.
           ∗ pc_a ↦ₐ[pc_p'] w
           ∗ r1 ↦ᵣ wr1 }}}.
   Proof.
-    iIntros (Hinstr Hfl Hvpc Hpca' Hne ϕ) "(>HPC & >Hpc_a & >Hr1) Hφ".
+    iIntros (Hinstr Hfl Hvpc Hpca' ϕ) "(>HPC & >Hpc_a & >Hr1) Hφ".
     iDestruct (map_of_regs_2 with "HPC Hr1") as "[Hmap %]".
     iApply (wp_Mov with "[$Hmap Hpc_a]"); eauto; simplify_map_eq; eauto.
     by unfold regs_of; rewrite !dom_insert; set_solver+.
@@ -248,7 +245,6 @@ Section cap_lang_rules.
     PermFlows pc_p pc_p' →
     isCorrectPC (inr ((pc_p,pc_g),pc_b,pc_e,pc_a)) →
     (pc_a + 1)%a = Some pc_a' →
-    PC ≠ r1 →
 
     {{{ ▷ PC ↦ᵣ inr ((pc_p,pc_g),pc_b,pc_e,pc_a)
         ∗ ▷ pc_a ↦ₐ[pc_p'] w
@@ -259,7 +255,7 @@ Section cap_lang_rules.
           ∗ pc_a ↦ₐ[pc_p'] w
           ∗ r1 ↦ᵣ inr ((pc_p,pc_g),pc_b,pc_e,pc_a) }}}.
   Proof.
-    iIntros (Hinstr Hfl Hvpc Hpca' Hne ϕ) "(>HPC & >Hpc_a & >Hr1) Hφ".
+    iIntros (Hinstr Hfl Hvpc Hpca' ϕ) "(>HPC & >Hpc_a & >Hr1) Hφ".
     iDestruct (map_of_regs_2 with "HPC Hr1") as "[Hmap %]".
     iApply (wp_Mov with "[$Hmap Hpc_a]"); eauto; simplify_map_eq; eauto.
     by unfold regs_of; rewrite !dom_insert; set_solver+.
